mechanization/theories/Core/Soundness/LogicalRelation.v
@@ -1,0 +1,1 @@
+From McPTS.Core.Soundness.LogicalRelation Require Export Core Lemmas.
