mechanization/theories/Core/Soundness/LogicalRelation/Lemmas.v
@@ -32,126 +32,39 @@ Proof.
     mauto.
 Qed.
 
-Add Parametric Morphism {P} (pred_P : PredicativeSig P) s a Γ A M R (H : per_sort_elem pred_P s R a a) : (glu_elem_top pred_P s a Γ A M)
-    with signature R ==> iff as glu_elem_top_morphism_iff4.
-Proof.
-  intros m m' Hmm' *.
-  split; intros []; econstructor; mauto 3;
-    pose proof (per_elem_then_per_top H Hmm') as Hmm'';
-    try (etransitivity; mauto 4);
-    intros;
-    specialize (Hmm'' (length Δ)) as [? []];
-    functional_read_rewrite_clear;
-    mauto.
-Qed.
-
-
-
-
-Add Parametric Morphism {P} (pred_P : PredicativeSig P) a Γ A M : (glu_elem_bot_unsorted pred_P a Γ A M)
-    with signature per_bot ==> iff as glu_elem_bot_unsorted_morphism_iff4.
-Proof.
-  intros m m' Hmm' *.
-  split; intros []; econstructor; mauto 3;
-    try (etransitivity; mauto 4);
-    intros;
-    specialize (Hmm' (length Δ)) as [? []];
-    functional_read_rewrite_clear;
-    mauto.
-Qed.
-
-Add Parametric Morphism {P} (pred_P : PredicativeSig P) s a Γ A M R (H : per_sort_elem pred_P s R a a) : (glu_elem_top pred_P s a Γ A M)
-    with signature R ==> iff as glu_elem_top_morphism_iff4.
-Proof.
-  intros m m' Hmm' *.
-  split; intros []; econstructor; mauto 3;
-    pose proof (per_elem_then_per_top H Hmm') as Hmm'';
-    try (etransitivity; mauto 4);
-    intros;
-    specialize (Hmm'' (length Δ)) as [? []];
-    functional_read_rewrite_clear;
-    mauto.
-Qed.
-
-Add Parametric Morphism {P} (pred_P : PredicativeSig P) s a Γ A M R (H : per_sort_elem pred_P s R a a) : (glu_elem_top pred_P s a Γ A M)
-    with signature R ==> iff as glu_elem_top_morphism_iff4.
-Proof.
-  intros m m' Hmm' *.
-  split; intros []; econstructor; mauto 3;
-    pose proof (per_elem_then_per_top H Hmm') as Hmm'';
-    try (etransitivity; mauto 4);
-    intros;
-    specialize (Hmm'' (length Δ)) as [? []];
-    functional_read_rewrite_clear;
-    mauto.
-Qed.
-
-
-
-
-
-Lemma glu_sort_elem_typ_unique_upto_exp_eq {P} (pred_P : PredicativeSig P) : forall {s s' a typ_rel typ_rel' exp_rel exp_rel' Γ A A'},
+Lemma glu_sort_elem_typ_unique_upto_exp_eq {P} (pred_P : PredicativeSig P) : forall {s a typ_rel typ_rel' exp_rel exp_rel' Γ A A'},
     {{ DG a ∈ glu_sort_elem pred_P s ↘ typ_rel ↘ exp_rel }} ->
-    {{ DG a ∈ glu_sort_elem pred_P s' ↘ typ_rel' ↘ exp_rel' }} ->
+    {{ DG a ∈ glu_sort_elem pred_P s ↘ typ_rel' ↘ exp_rel' }} ->
     {{ Γ ⊢ A ® typ_rel }} ->
     {{ Γ ⊢ A' ® typ_rel' }} ->
-    {{ Γ ⊢ A ≈ A' }}.
+    {{ Γ ⊢ A ≈ A' : Sort@s }}.
 Proof with mautosolve 4.
   intros.
   assert {{ Γ ⊢ A ® glu_typ_top pred_P s a }} as [] by mauto 3.
-  assert {{ Γ ⊢ A' ® glu_typ_top pred_P s' a }} as [] by mauto 3.
+  assert {{ Γ ⊢ A' ® glu_typ_top pred_P s a }} as [] by mauto 3.
   match_by_head (@per_top_typ P) ltac:(fun H => destruct (H (length Γ)) as [V []]).
   clear_dups.
   functional_read_rewrite_clear.
   assert {{ Γ ⊢ A[Id] ≈ V : Sort@s }} by mauto 4.
-  assert {{ Γ ⊢ A[Id] ≈ V }} by mauto 2.
-  assert {{ Γ ⊢ A ≈ A[Id] }} by mauto 4.
-  assert {{ Γ ⊢ A ≈ V }} by (etransitivity; mauto 2).
-  
-  assert {{ Γ ⊢ A'[Id] ≈ V : Sort@s' }} by mauto 4.
-  assert {{ Γ ⊢ A'[Id] ≈ V }} by mauto 2.
-  assert {{ Γ ⊢ A' ≈ A'[Id] }} by mauto 4.
-  assert {{ Γ ⊢ A' ≈ V }} by (etransitivity; mauto 2).
-  
-  transitivity V; mauto 2.
+  assert {{ Γ ⊢ A ≈ A[Id] : Sort@s }} by mauto 3.
+  assert {{ Γ ⊢ A ≈ V : Sort@s }} by (etransitivity; mauto 3).
+  assert {{ Γ ⊢ A'[Id] ≈ V : Sort@s }} by mauto 4.
+  assert {{ Γ ⊢ A' ≈ A'[Id] : Sort@s }} by mauto 3.
+  assert {{ Γ ⊢ A' ≈ V : Sort@s }} by (etransitivity; mauto 3).
+  etransitivity; mauto 3.
 Qed.
 
 #[export]
 Hint Resolve glu_sort_elem_typ_unique_upto_exp_eq : mcpts.
 
-(* Lemma glu_sort_elem_typ_unique_upto_exp_eq_ge : forall {i j a P P' El El' Γ A A'}, *)
-(*     i <= j -> *)
-(*     {{ DG a ∈ glu_sort_elem i ↘ P ↘ El }} -> *)
-(*     {{ DG a ∈ glu_sort_elem j ↘ P' ↘ El' }} -> *)
-(*     {{ Γ ⊢ A ® P }} -> *)
-(*     {{ Γ ⊢ A' ® P' }} -> *)
-(*     {{ Γ ⊢ A ≈ A' : Type@j }}. *)
-(* Proof with mautosolve 4. *)
-(*   intros. *)
-(*   replace j with (max i j) by lia... *)
-(* Qed. *)
-
-(* #[export] *)
-(* Hint Resolve glu_sort_elem_typ_unique_upto_exp_eq_ge : mcpts. *)
-
-Lemma glu_sort_elem_typ_unique_upto_exp_eq' {P} (pred_P : PredicativeSig P) : forall {s a typ_rel exp_rel Γ A A'},
-    {{ DG a ∈ glu_sort_elem pred_P s ↘ typ_rel ↘ exp_rel }} ->
-    {{ Γ ⊢ A ® typ_rel }} ->
-    {{ Γ ⊢ A' ® typ_rel }} ->
-    {{ Γ ⊢ A ≈ A' }}.
-Proof. mautosolve 4. Qed.
-
-#[export]
-Hint Resolve glu_sort_elem_typ_unique_upto_exp_eq' : mcpts.
-
 
 Lemma glu_sort_elem_per_sort_elem_typ_escape {P} (pred_P : PredicativeSig P) : forall {s a a' elem_rel typ_rel typ_rel' exp_rel exp_rel' Γ A A'},
     {{ DF a ≈ a' ∈ per_sort_elem pred_P s ↘ elem_rel }} ->
-    {{ DG a ∈ glu_sort_elem pred_P s  ↘ typ_rel ↘ exp_rel }} ->
+    {{ DG a ∈ glu_sort_elem pred_P s ↘ typ_rel ↘ exp_rel }} ->
     {{ DG a' ∈ glu_sort_elem pred_P s ↘ typ_rel' ↘ exp_rel' }} ->
     {{ Γ ⊢ A ® typ_rel }} ->
     {{ Γ ⊢ A' ® typ_rel' }} ->
-    {{ Γ ⊢ A ≈ A' }}.
+    {{ Γ ⊢ A ≈ A' : Sort@s }}.
 Proof with mautosolve 4.
   simpl in *.
   intros * Hper Hglu Hglu' HA HA'.
@@ -162,13 +75,14 @@ Qed.
 #[export]
 Hint Resolve glu_sort_elem_per_sort_elem_typ_escape : mcpts.
 
+
 Lemma glu_sort_elem_per_sort_typ_escape {P} (pred_P : PredicativeSig P) : forall {s a a' typ_rel typ_rel' exp_rel exp_rel' Γ A A'},
     {{ Dom a ≈ a' ∈ per_sort pred_P s }} ->
     {{ DG a ∈ glu_sort_elem pred_P s ↘ typ_rel ↘ exp_rel }} ->
     {{ DG a' ∈ glu_sort_elem pred_P s ↘ typ_rel' ↘ exp_rel' }} ->
     {{ Γ ⊢ A ® typ_rel }} ->
     {{ Γ ⊢ A' ® typ_rel' }} ->
-    {{ Γ ⊢ A ≈ A' }}.
+    {{ Γ ⊢ A ≈ A' : Sort@s }}.
 Proof.
   intros * [] **...
   mauto 4.
@@ -177,17 +91,19 @@ Qed.
 #[export]
 Hint Resolve glu_sort_elem_per_sort_typ_escape : mcpts.
 
-Lemma glu_sort_elem_exp_unique_upto_exp_eq {P} (pred_P : PredicativeSig P) : forall {s s' a typ_rel typ_rel' exp_rel exp_rel' Γ A A' M M' m},
+
+
+Lemma glu_sort_elem_exp_unique_upto_exp_eq {P} (pred_P : PredicativeSig P) : forall {s a typ_rel typ_rel' exp_rel exp_rel' Γ A A' M M' m},
     {{ DG a ∈ glu_sort_elem pred_P s ↘ typ_rel ↘ exp_rel }} ->
-    {{ DG a ∈ glu_sort_elem pred_P s' ↘ typ_rel' ↘ exp_rel' }} ->
+    {{ DG a ∈ glu_sort_elem pred_P s ↘ typ_rel' ↘ exp_rel' }} ->
     {{ Γ ⊢ M : A ® m ∈ exp_rel }} ->
     {{ Γ ⊢ M' : A' ® m ∈ exp_rel' }} ->
     {{ Γ ⊢ M ≈ M' : A }}.
 Proof.
   intros.
   assert {{ Γ ⊢ M : A ® m ∈ glu_elem_top pred_P s a }} as [] by mauto 3.
-  assert {{ Γ ⊢ M' : A' ® m ∈ glu_elem_top pred_P s' a }} as [] by mauto 3.
-  assert {{ Γ ⊢ A ≈ A' }} by mauto 3.
+  assert {{ Γ ⊢ M' : A' ® m ∈ glu_elem_top pred_P s a }} as [] by mauto 3.
+  assert {{ Γ ⊢ A ≈ A' : Sort@s }} by mauto 3.
   match_by_head (@per_top P) ltac:(fun H => destruct (H (length Γ)) as [W []]).
   clear_dups.
   assert {{ Γ ⊢ M[Id] ≈ W : A[Id] }} by mauto 4.
@@ -203,18 +119,18 @@ Proof.
 Qed.
 
 #[export]
- Hint Resolve glu_sort_elem_exp_unique_upto_exp_eq : mcpts.
+Hint Resolve glu_sort_elem_exp_unique_upto_exp_eq : mcpts.
 
-Lemma glu_sort_elem_exp_unique_upto_exp_eq' {P} (pred_P : PredicativeSig P) : forall {s a typ_rel exp_rel Γ M M' m A},
+Lemma glu_sort_elem_exp_unique_upto_exp_eq' {P} (pred_P : PredicativeSig P) : forall {s a typ_rel exp_rel Γ A A' M M' m},
     {{ DG a ∈ glu_sort_elem pred_P s ↘ typ_rel ↘ exp_rel }} ->
     {{ Γ ⊢ M : A ® m ∈ exp_rel }} ->
-    {{ Γ ⊢ M' : A ® m ∈ exp_rel }} ->
+    {{ Γ ⊢ M' : A' ® m ∈ exp_rel }} ->
     {{ Γ ⊢ M ≈ M' : A }}.
 Proof. mautosolve 4. Qed.
 
-
 #[export]
 Hint Resolve glu_sort_elem_exp_unique_upto_exp_eq' : mcpts.
+
 
 Lemma glu_sort_elem_per_sort_typ_iff {P} (pred_P : PredicativeSig P) : forall {s a a' typ_rel typ_rel' exp_rel exp_rel'},
     {{ Dom a ≈ a' ∈ per_sort pred_P s }} ->
@@ -229,491 +145,91 @@ Proof.
 Qed.
 
 
-    
-(* Section glu_sort_elem_cumulativity. *)
-(*   #[local] *)
-(*   Lemma glu_sort_elem_cumulativity_ge : forall {i j a P P' El El'}, *)
-(*       i <= j -> *)
-(*       {{ DG a ∈ glu_sort_elem i ↘ P ↘ El }} -> *)
-(*       {{ DG a ∈ glu_sort_elem j ↘ P' ↘ El' }} -> *)
-(*       (forall Γ A, {{ Γ ⊢ A ® P }} -> {{ Γ ⊢ A ® P' }}) /\ *)
-(*         (forall Γ A M m, {{ Γ ⊢ M : A ® m ∈ El }} -> {{ Γ ⊢ M : A ® m ∈ El' }}) /\ *)
-(*         (forall Γ A M m, {{ Γ ⊢ A ® P }} -> {{ Γ ⊢ M : A ® m ∈ El' }} -> {{ Γ ⊢ M : A ® m ∈ El }}). *)
-(*   Proof with mautosolve 4. *)
-(*     simpl. *)
-(*     intros * Hge Hglu Hglu'. gen El' P' j. *)
-(*     induction Hglu using glu_sort_elem_ind; repeat split; intros; *)
-(*       try assert {{ DF a ≈ a ∈ per_sort_elem j ↘ in_rel }} by mauto 2; *)
-(*       invert_glu_sort_elem Hglu'; *)
-(*       handle_functional_glu_sort_elem; *)
-(*       simpl in *; *)
-(*       try solve [repeat split; intros; destruct_conjs; mauto 2 | intuition mauto 3]. *)
-
-(*     - rename x into IP'. *)
-(*       rename x0 into IEl'. *)
-(*       rename x1 into OP'. *)
-(*       rename x2 into OEl'. *)
-(*       destruct_by_head pi_glu_typ_pred. *)
-(*       econstructor; intros; mauto 4. *)
-(*       + assert {{ Δ ⊢ IT[σ] ® IP }} by mauto. *)
-(*         enough (forall Γ A, {{ Γ ⊢ A ® IP }} -> {{ Γ ⊢ A ® IP' }}) by mauto 4. *)
-(*         eapply proj1... *)
-(*       + match_by_head per_sort_elem ltac:(fun H => directed invert_per_sort_elem H). *)
-(*         apply_relation_equivalence. *)
-(*         destruct_rel_mod_eval. *)
-(*         handle_per_sort_elem_irrel. *)
-(*         assert (forall Γ A, {{ Γ ⊢ A ® OP m equiv_m }} -> {{ Γ ⊢ A ® OP' m equiv_m }}) by (eapply proj1; mauto). *)
-(*         enough {{ Δ ⊢ OT[σ,,M] ® OP m equiv_m }} by mauto. *)
-(*         enough {{ Δ ⊢ M : IT[σ] ® m ∈ IEl }} by mauto. *)
-(*         eapply IHHglu... *)
-(*     - rename x into IP'. *)
-(*       rename x0 into IEl'. *)
-(*       rename x1 into OP'. *)
-(*       rename x2 into OEl'. *)
-(*       destruct_by_head pi_glu_exp_pred. *)
-(*       handle_per_sort_elem_irrel. *)
-(*       econstructor; intros; mauto 4. *)
-(*       + enough (forall Γ A, {{ Γ ⊢ A ® IP }} -> {{ Γ ⊢ A ® IP' }}) by mauto 4. *)
-(*         eapply proj1... *)
-(*       + match_by_head per_sort_elem ltac:(fun H => directed invert_per_sort_elem H). *)
-(*         handle_per_sort_elem_irrel. *)
-(*         destruct_rel_mod_eval. *)
-(*         destruct_rel_mod_app. *)
-(*         handle_per_sort_elem_irrel. *)
-(*         eexists; split; mauto 4. *)
-(*         assert (forall Γ A M m, {{ Γ ⊢ M : A ® m ∈ OEl n equiv_n }} -> {{ Γ ⊢ M : A ® m ∈ OEl' n equiv_n }}) by (eapply proj1, proj2; mauto 4). *)
-(*         enough {{ Δ ⊢ M[σ] N : OT[σ,,N] ® fa ∈ OEl n equiv_n }} by mauto 4. *)
-(*         assert {{ Δ ⊢ N : IT[σ] ® n ∈ IEl }} by (eapply IHHglu; mauto 3). *)
-(*         assert (exists mn, {{ $| m & n |↘ mn }} /\ {{ Δ ⊢ M[σ] N : OT[σ,,N] ® mn ∈ OEl n equiv_n }}) by mauto 4. *)
-(*         destruct_conjs. *)
-(*         functional_eval_rewrite_clear... *)
-(*     - rename x into IP'. *)
-(*       rename x0 into IEl'. *)
-(*       rename x1 into OP'. *)
-(*       rename x2 into OEl'. *)
-(*       destruct_by_head pi_glu_typ_pred. *)
-(*       destruct_by_head pi_glu_exp_pred. *)
-(*       handle_per_sort_elem_irrel. *)
-(*       econstructor; intros; mauto. *)
-(*       match_by_head per_sort_elem ltac:(fun H => directed invert_per_sort_elem H). *)
-(*       handle_per_sort_elem_irrel. *)
-(*       destruct_rel_mod_eval. *)
-(*       destruct_rel_mod_app. *)
-(*       handle_per_sort_elem_irrel. *)
-(*       match goal with *)
-(*       | _: {{ ⟦ B ⟧ ρ ↦ n ↘ ^?a }} |- _ => *)
-(*           rename a into b *)
-(*       end. *)
-(*       eexists; split; mauto 4. *)
-(*       assert (forall Γ A M m, {{ Γ ⊢ A ® OP n equiv_n }} -> {{ Γ ⊢ M : A ® m ∈ OEl' n equiv_n }} -> {{ Γ ⊢ M : A ® m ∈ OEl n equiv_n }}) by (eapply proj2, proj2; eauto 3). *)
-(*       assert {{ Δ ⊢ OT[σ,,N] ® OP n equiv_n }} by mauto 4. *)
-(*       enough {{ Δ ⊢ M[σ] N : OT[σ,,N] ® fa ∈ OEl' n equiv_n }} by mauto 4. *)
-(*       assert {{ Δ ⊢ N : IT[σ] ® n ∈ IEl' }} by (eapply IHHglu; mauto 3). *)
-(*       assert {{ Δ ⊢ IT[σ] ® IP' }} by (eapply glu_sort_elem_trm_typ; mauto 2). *)
-(*       assert {{ Δ ⊢ IT0[σ] ® IP' }} by mauto 2. *)
-(*       assert {{ Δ ⊢ IT[σ] ≈ IT0[σ] : Type@j }} as HITeq by mauto 2. *)
-(*       assert {{ Δ ⊢ N : IT0[σ] ® n ∈ IEl' }} by (rewrite <- HITeq; mauto 3). *)
-(*       assert (exists mn, {{ $| m & n |↘ mn }} /\ {{ Δ ⊢ M[σ] N : OT0[σ,,N] ® mn ∈ OEl' n equiv_n }}) by mauto 3. *)
-(*       destruct_conjs. *)
-(*       functional_eval_rewrite_clear. *)
-(*       assert {{ DG b ∈ glu_sort_elem j ↘ OP' n equiv_n ↘ OEl' n equiv_n }} by mauto 3. *)
-(*       assert {{ Δ ⊢ OT0[σ,,N] ® OP' n equiv_n }} by (eapply glu_sort_elem_trm_typ; mauto 3). *)
-(*       enough {{ Δ ⊢ OT[σ,,N] ≈ OT0[σ,,N] : Type@j }} as ->... *)
-
-(*     - invert_glu_rel1. *)
-(*       econstructor; intros; firstorder mauto 3. *)
-(*     - invert_glu_rel1. *)
-(*       handle_per_sort_elem_irrel. *)
-
-(*       econstructor; intros; firstorder mauto 3. *)
-(*       destruct_glu_eq; econstructor; firstorder mauto 3. *)
-(*     - repeat invert_glu_rel1. *)
-(*       handle_per_sort_elem_irrel. *)
-
-(*       econstructor; intros; firstorder mauto 3. *)
-(*       assert {{ Γ ⊢w Id : Γ }} by mauto 4. *)
-(*       assert (P Γ {{{ B[Id] }}}) as HB by mauto 3. *)
-(*       bulky_rewrite_in HB. *)
-(*       assert (P0 Γ B) as HB' by firstorder. *)
-(*       assert (P0 Γ {{{ B0[Id] }}}) as HB0 by mauto 3. *)
-(*       bulky_rewrite_in HB0. *)
-(*       assert {{ Γ ⊢ B0 ≈ B : Type@j }} by mauto 3. *)
-(*       assert (El Γ {{{ B[Id] }}} {{{ M0[Id] }}} m) as HM0 by mauto 3. *)
-(*       bulky_rewrite_in HM0. *)
-(*       assert (El0 Γ B M0 m) as HM0' by firstorder. *)
-(*       assert (El Γ {{{ B[Id] }}} {{{ N[Id] }}} n) as HN by mauto 3. *)
-(*       bulky_rewrite_in HN. *)
-(*       assert (El0 Γ B N n) as HN' by firstorder. *)
-(*       assert (El0 Γ {{{ B0[Id] }}} {{{ M[Id] }}} m) as HM by mauto 3. *)
-(*       bulky_rewrite_in HM. *)
-(*       assert (El0 Γ {{{ B0[Id] }}} {{{ N0[Id] }}} n) as HN0 by mauto 3. *)
-(*       bulky_rewrite_in HN0. *)
-(*       assert {{ Γ ⊢ M0 ≈ M : B }} by mauto 3. *)
-(*       assert {{ Γ ⊢ N ≈ N0 : B }} by mauto 3. *)
-
-(*       destruct_glu_eq; econstructor; apply_equiv_left; mauto 3. *)
-(*       + bulky_rewrite. *)
-(*         eapply wf_exp_eq_conv'; [econstructor |]; mauto 3. *)
-(*         transitivity M; mauto 3. *)
-(*         bulky_rewrite. *)
-(*       + transitivity M; mauto 3. *)
-(*         transitivity M''; mauto 3. *)
-(*         transitivity N0; mauto 3. *)
-(*       + intros. *)
-(*         assert (P Δ {{{ B[σ] }}}) by mauto 3. *)
-(*         assert {{ Δ ⊢ B0[σ] ≈ B[σ] : Type@j }} by mauto 3. *)
-(*         assert {{ Γ ⊢ M'' ≈ M0 : B }} by (transitivity M; mauto 3). *)
-(*         assert {{ Δ ⊢ M''[σ] ≈ M0[σ] : B[σ] }} by mauto 4. *)
-(*         assert (El0 Δ {{{ B0[σ] }}} {{{M''[σ]}}} m') as HEl0 by mauto 3. *)
-(*         bulky_rewrite_in HEl0. *)
-(*         firstorder. *)
-
-(*     - destruct_by_head neut_glu_exp_pred. *)
-(*       econstructor; mauto. *)
-(*       destruct_by_head neut_glu_typ_pred. *)
-(*       econstructor... *)
-(*     - destruct_by_head neut_glu_exp_pred. *)
-(*       econstructor... *)
-(*   Qed. *)
-(* End glu_sort_elem_cumulativity. *)
-
-(* Corollary glu_sort_elem_typ_cumu_ge : forall {i j a P P' El El' Γ A}, *)
-(*     i <= j -> *)
-(*     {{ DG a ∈ glu_sort_elem i ↘ P ↘ El }} -> *)
-(*     {{ DG a ∈ glu_sort_elem j ↘ P' ↘ El' }} -> *)
-(*     {{ Γ ⊢ A ® P }} -> *)
-(*     {{ Γ ⊢ A ® P' }}. *)
-(* Proof. *)
-(*   intros. *)
-(*   eapply glu_sort_elem_cumulativity_ge; mauto 4. *)
-(* Qed. *)
-
-(* Corollary glu_sort_elem_typ_cumu_max_left : forall {i j a P P' El El' Γ A}, *)
-(*     {{ DG a ∈ glu_sort_elem i ↘ P ↘ El }} -> *)
-(*     {{ DG a ∈ glu_sort_elem (max i j) ↘ P' ↘ El' }} -> *)
-(*     {{ Γ ⊢ A ® P }} -> *)
-(*     {{ Γ ⊢ A ® P' }}. *)
-(* Proof. *)
-(*   intros. *)
-(*   assert (i <= max i j) by lia. *)
-(*   eapply glu_sort_elem_typ_cumu_ge; mauto 4. *)
-(* Qed. *)
-
-(* Corollary glu_sort_elem_typ_cumu_max_right : forall {i j a P P' El El' Γ A}, *)
-(*     {{ DG a ∈ glu_sort_elem j ↘ P ↘ El }} -> *)
-(*     {{ DG a ∈ glu_sort_elem (max i j) ↘ P' ↘ El' }} -> *)
-(*     {{ Γ ⊢ A ® P }} -> *)
-(*     {{ Γ ⊢ A ® P' }}. *)
-(* Proof. *)
-(*   intros. *)
-(*   assert (j <= max i j) by lia. *)
-(*   eapply glu_sort_elem_typ_cumu_ge; mauto 4. *)
-(* Qed. *)
-
-(* Corollary glu_sort_elem_exp_cumu_ge : forall {i j a P P' El El' Γ A M m}, *)
-(*     i <= j -> *)
-(*     {{ DG a ∈ glu_sort_elem i ↘ P ↘ El }} -> *)
-(*     {{ DG a ∈ glu_sort_elem j ↘ P' ↘ El' }} -> *)
-(*     {{ Γ ⊢ M : A ® m ∈ El }} -> *)
-(*     {{ Γ ⊢ M : A ® m ∈ El' }}. *)
-(* Proof. *)
-(*   intros. gen m M A Γ. *)
-(*   eapply glu_sort_elem_cumulativity_ge; mauto 4. *)
-(* Qed. *)
-
-(* Corollary glu_sort_elem_exp_cumu_max_left : forall {i j a P P' El El' Γ A M m}, *)
-(*     {{ DG a ∈ glu_sort_elem i ↘ P ↘ El }} -> *)
-(*     {{ DG a ∈ glu_sort_elem (max i j) ↘ P' ↘ El' }} -> *)
-(*     {{ Γ ⊢ M : A ® m ∈ El }} -> *)
-(*     {{ Γ ⊢ M : A ® m ∈ El' }}. *)
-(* Proof. *)
-(*   intros. *)
-(*   assert (i <= max i j) by lia. *)
-(*   eapply glu_sort_elem_exp_cumu_ge; mauto 4. *)
-(* Qed. *)
-
-(* Corollary glu_sort_elem_exp_cumu_max_right : forall {i j a P P' El El' Γ A M m}, *)
-(*     {{ DG a ∈ glu_sort_elem j ↘ P ↘ El }} -> *)
-(*     {{ DG a ∈ glu_sort_elem (max i j) ↘ P' ↘ El' }} -> *)
-(*     {{ Γ ⊢ M : A ® m ∈ El }} -> *)
-(*     {{ Γ ⊢ M : A ® m ∈ El' }}. *)
-(* Proof. *)
-(*   intros. *)
-(*   assert (j <= max i j) by lia. *)
-(*   eapply glu_sort_elem_exp_cumu_ge; mauto 4. *)
-(* Qed. *)
-
-(* Corollary glu_sort_elem_exp_lower :  forall {i j a P P' El El' Γ A M m}, *)
-(*     i <= j -> *)
-(*     {{ DG a ∈ glu_sort_elem i ↘ P ↘ El }} -> *)
-(*     {{ DG a ∈ glu_sort_elem j ↘ P' ↘ El' }} -> *)
-(*     {{ Γ ⊢ A ® P }} -> *)
-(*     {{ Γ ⊢ M : A ® m ∈ El' }} -> *)
-(*     {{ Γ ⊢ M : A ® m ∈ El }}. *)
-(* Proof. *)
-(*   intros * ? ? ?. gen m M A Γ. *)
-(*   eapply glu_sort_elem_cumulativity_ge; mauto 4. *)
-(* Qed. *)
-
-(* Corollary glu_sort_elem_exp_lower_max_left :  forall {i j a P P' El El' Γ A M m}, *)
-(*     {{ DG a ∈ glu_sort_elem i ↘ P ↘ El }} -> *)
-(*     {{ DG a ∈ glu_sort_elem (max i j) ↘ P' ↘ El' }} -> *)
-(*     {{ Γ ⊢ A ® P }} -> *)
-(*     {{ Γ ⊢ M : A ® m ∈ El' }} -> *)
-(*     {{ Γ ⊢ M : A ® m ∈ El }}. *)
-(* Proof. *)
-(*   intros. *)
-(*   assert (i <= max i j) by lia. *)
-(*   eapply glu_sort_elem_exp_lower; mauto 4. *)
-(* Qed. *)
-
-(* Corollary glu_sort_elem_exp_lower_max_right :  forall {i j a P P' El El' Γ A M m}, *)
-(*     {{ DG a ∈ glu_sort_elem j ↘ P ↘ El }} -> *)
-(*     {{ DG a ∈ glu_sort_elem (max i j) ↘ P' ↘ El' }} -> *)
-(*     {{ Γ ⊢ A ® P }} -> *)
-(*     {{ Γ ⊢ M : A ® m ∈ El' }} -> *)
-(*     {{ Γ ⊢ M : A ® m ∈ El }}. *)
-(* Proof. *)
-(*   intros. *)
-(*   assert (j <= max i j) by lia. *)
-(*   eapply glu_sort_elem_exp_lower; mauto 4. *)
-(* Qed. *)
-
-Lemma glu_sort_elem_exp_conv {P} (pred_P : PredicativeSig P) : forall {s a a' typ_rel typ_rel' exp_rel exp_rel' Γ A M m},
-    {{ Dom a ≈ a' ∈ per_sort pred_P s }} ->
+Lemma glu_sort_elem_per_typ_iff {P} (pred_P : PredicativeSig P) : forall {s a a' typ_rel typ_rel' exp_rel exp_rel'},
+    {{ Dom a ≈ a' ∈ per_typ pred_P }} ->
     {{ DG a ∈ glu_sort_elem pred_P s ↘ typ_rel ↘ exp_rel }} ->
     {{ DG a' ∈ glu_sort_elem pred_P s ↘ typ_rel' ↘ exp_rel' }} ->
-    {{ Γ ⊢ M : A ® m ∈ exp_rel }} ->
-    {{ Γ ⊢ A ® typ_rel' }} ->
-    {{ Γ ⊢ M : A ® m ∈ exp_rel' }}.
+    (typ_rel <∙> typ_rel') /\ (exp_rel <∙> exp_rel').
 Proof.
-  intros * [] Hglu Hglu' ER TR.
-  
-  assert ((typ_rel <∙> typ_rel') /\ (exp_rel <∙> exp_rel')) by (eapply glu_sort_elem_per_sort_typ_iff; mauto 3).
+  intros * Hper **.
+  assert (per_sort pred_P s a a) by mauto 2.
+  unfold per_sort in H1.
+  unfold per_typ in Hper.
   destruct_conjs.
-  eapply H1; mauto 2.
+  assert (per_sort_elem pred_P s Hper a a') by mauto 2.
+  assert (per_sort pred_P s a a') by mauto 3.
+  eapply glu_sort_elem_per_sort_typ_iff; mauto 2.
 Qed.
 
 
-(*   (* assert {{ Dom a ≈ a' ∈ per_sort (max i k) }} as Haa' by (eexists; mauto using per_sort_elem_cumu_max_right). *) *)
-(*   assert (exists P El, {{ DG a ∈ glu_sort_elem (max i k) ↘ P ↘ El }}) as [Pik [Elik]] by mauto using glu_sort_elem_cumu_max_left. *)
-(*   assert {{ DG a' ∈ glu_sort_elem (max i k) ↘ Pik ↘ Elik }} by (setoid_rewrite <- Haa'; eassumption). *)
-(*   assert {{ Γ ⊢ M : A ® m ∈ Elik }} by (eapply glu_sort_elem_exp_cumu_max_left; [| | eassumption]; eassumption). *)
-(*   assert (exists P El, {{ DG a' ∈ glu_sort_elem (max j (max i k)) ↘ P ↘ El }}) as [Ptop [Eltop]] by mauto using glu_sort_elem_cumu_max_right. *)
-(*   assert {{ Γ ⊢ M : A ® m ∈ Eltop }} by (eapply glu_sort_elem_exp_cumu_max_right; [| | eassumption]; eassumption). *)
-(*   eapply glu_sort_elem_exp_lower_max_left; mauto. *)
+(* Lemma glu_sort_elem_exp_conv {P} (pred_P : PredicativeSig P) : forall {s a a' typ_rel typ_rel' exp_rel exp_rel' Γ A M m}, *)
+(*     {{ Dom a ≈ a' ∈ per_sort pred_P s }} -> *)
+(*     {{ DG a ∈ glu_sort_elem pred_P s ↘ typ_rel ↘ exp_rel }} -> *)
+(*     {{ DG a' ∈ glu_sort_elem pred_P s ↘ typ_rel' ↘ exp_rel' }} -> *)
+(*     {{ Γ ⊢ M : A ® m ∈ exp_rel }} -> *)
+(*     {{ Γ ⊢ A ® typ_rel' }} -> *)
+(*     {{ Γ ⊢ M : A ® m ∈ exp_rel' }}. *)
+(* Proof. *)
+(*   intros * [] ? ? ? ?. *)
+(*   assert ((typ_rel <∙> typ_rel') /\ (exp_rel <∙> exp_rel')) by (eapply glu_sort_elem_per_sort_typ_iff; mauto 3). *)
+(*   destruct_conjs. *)
+(*   apply_predicate_equivalence. *)
+(*   eassumption. *)
 (* Qed. *)
 
-
-Lemma glu_sort_elem_exp_conv' {P} (pred_P : PredicativeSig P) : forall {s a typ_rel typ_rel' exp_rel exp_rel' Γ A M m},
-    {{ DG a ∈ glu_sort_elem pred_P s ↘ typ_rel ↘ exp_rel }} ->
-    {{ DG a ∈ glu_sort_elem pred_P s ↘ typ_rel' ↘ exp_rel' }} ->
+Lemma glu_sort_elem_exp_conv {P} (pred_P : PredicativeSig P) : forall {s1 s2 s3 a a' typ_rel typ_rel' exp_rel exp_rel' Γ A M m},
+    {{ Dom a ≈ a' ∈ per_sort pred_P s1 }} ->
+    {{ DG a ∈ glu_sort_elem pred_P s2 ↘ typ_rel ↘ exp_rel }} ->
+    {{ DG a' ∈ glu_sort_elem pred_P s3 ↘ typ_rel' ↘ exp_rel' }} ->
     {{ Γ ⊢ M : A ® m ∈ exp_rel }} ->
     {{ Γ ⊢ A ® typ_rel' }} ->
     {{ Γ ⊢ M : A ® m ∈ exp_rel' }}.
 Proof.
-  intros.
-  eapply glu_sort_elem_exp_conv; only 2: exact H; eauto.
-  mauto 2.
+  intros * [] ? ? ? ?.
+
+  assert (per_typ_elem pred_P x a a') by mauto 2.
+  assert (per_sort_elem pred_P s2 x a a').
+  {
+    assert (per_sort pred_P s2 a a) by mauto 2.
+    destruct H5 as [R2 ?].
+    mauto.
+  }
+
+  assert (per_sort_elem pred_P s3 x a' a).
+  {
+    assert (per_sort pred_P s3 a' a') by mauto 2.
+    destruct H6 as [R3 ?].
+    symmetry in H4.
+    mauto.
+  }
+  assert (glu_sort_elem pred_P s2 typ_rel exp_rel a') by (eapply glu_sort_elem_resp_per_sort; mauto 3).
+  assert (glu_sort_elem pred_P s3 typ_rel' exp_rel' a) by (eapply glu_sort_elem_resp_per_sort; mauto 3).
+
+  invert_glu_sort_elem H0.
+  - invert_glu_sort_elem H9.
+    unfold sort_glu_exp_pred' in *.
+    unfold glu_sort_typ_rec in *.                                  
+    apply_predicate_equivalence.
+    destruct_conjs.
+    repeat eexists; mauto 2.
+
+  - invert_glu_sort_elem H12.
+    assert ((typ_rel <∙> typ_rel') /\ (el_rel <∙> exp_rel')) by (eapply functional_glu_sort_elem; mauto 2).
+    destruct_conjs.
+    eapply H18.
+    eassumption.
+
+  - invert_glu_sort_elem H10.
+    simpl_glu_rel.
+    econstructor; mauto 2.
+    econstructor; mauto 2.
+
+  - invert_glu_sort_elem H9.
+    simpl_glu_rel.
+    split; mauto 2.
+    eapply glu_nat_rule_irrelevance; mauto 2.
 Qed.
 
-
-(* Lemma glu_sort_elem_per_subtyp_typ_escape : forall {i a a' P P' El El' Γ A A'}, *)
-(*     {{ Sub a <: a' at i }} -> *)
-(*     {{ DG a ∈ glu_sort_elem i ↘ P ↘ El }} -> *)
-(*     {{ DG a' ∈ glu_sort_elem i ↘ P' ↘ El' }} -> *)
-(*     {{ Γ ⊢ A ® P }} -> *)
-(*     {{ Γ ⊢ A' ® P' }} -> *)
-(*     {{ Γ ⊢ A ⊆ A' }}. *)
-(* Proof. *)
-(*   intros * Hsubtyp Hglu Hglu' HA HA'. *)
-(*   gen A' A Γ. gen El' El P' P. *)
-(*   induction Hsubtyp using per_subtyp_ind; intros; subst; *)
-(*     saturate_refl_for per_sort_elem; *)
-(*     try solve [simpl in *; bulky_rewrite; mauto 3]; *)
-(*     invert_glu_sort_elem Hglu; *)
-(*     handle_functional_glu_sort_elem; *)
-(*     handle_per_sort_elem_irrel; *)
-(*     destruct_by_head pi_glu_typ_pred; *)
-(*     saturate_glu_by_per; *)
-(*     invert_glu_sort_elem Hglu'; *)
-(*     handle_functional_glu_sort_elem. *)
-(*   - bulky_rewrite. *)
-(*     mauto 3. *)
-(*   - destruct_by_head pi_glu_typ_pred. *)
-(*     rename x into IP. rename x0 into IEl. rename x1 into OP. rename x2 into OEl. *)
-(*     rename A0 into A'. rename IT0 into IT'. rename OT0 into OT'. *)
-(*     rename x3 into OP'. rename x4 into OEl'. *)
-(*     assert {{ Γ ⊢ IT ® IP }}. *)
-(*     { *)
-(*       assert {{ Γ ⊢ IT[Id] ® IP }} by mauto 4. *)
-(*       simpl in *. *)
-(*       autorewrite with mcpts in *; mauto 3. *)
-(*     } *)
-(*     assert {{ Γ ⊢ IT' ® IP }}. *)
-(*     { *)
-(*       assert {{ Γ ⊢ IT'[Id] ® IP }} by mauto 4. *)
-(*       simpl in *. *)
-(*       autorewrite with mcpts in *; mauto 3. *)
-(*     } *)
-(*     do 2 bulky_rewrite1. *)
-(*     assert {{ Γ ⊢ IT ≈ IT' : Type@i }} by mauto 4. *)
-(*     enough {{ Γ, IT' ⊢ OT ⊆ OT' }} by mauto 3. *)
-(*     assert {{ Dom ⇑! a (length Γ) ≈ ⇑! a' (length Γ) ∈ in_rel }} as equiv_len_len' by (eapply per_bot_then_per_elem; mauto 4). *)
-(*     assert {{ Dom ⇑! a (length Γ) ≈ ⇑! a (length Γ) ∈ in_rel }} as equiv_len_len by (eapply per_bot_then_per_elem; mauto 4). *)
-(*     assert {{ Dom ⇑! a' (length Γ) ≈ ⇑! a' (length Γ) ∈ in_rel }} as equiv_len'_len' by (eapply per_bot_then_per_elem; mauto 4). *)
-(*     handle_per_sort_elem_irrel. *)
-(*     match_by_head per_sort_elem ltac:(fun H => directed invert_per_sort_elem H). *)
-(*     apply_relation_equivalence. *)
-(*     destruct_rel_mod_eval. *)
-(*     handle_per_sort_elem_irrel. *)
-(*     match goal with *)
-(*     | _: {{ ⟦ B ⟧ ρ ↦ ⇑! a (length Γ) ↘ ^?a0 }}, *)
-(*         _: {{ ⟦ B' ⟧ ρ' ↦ ⇑! a' (length Γ) ↘ ^?a0' }} |- _ => *)
-(*         rename a0 into b; *)
-(*         rename a0' into b' *)
-(*     end. *)
-(*     assert {{ DG b ∈ glu_sort_elem i ↘ OP d{{{ ⇑! a (length Γ) }}} equiv_len_len ↘ OEl d{{{ ⇑! a (length Γ) }}} equiv_len_len }} by mauto 4. *)
-(*     assert {{ DG b' ∈ glu_sort_elem i ↘ OP' d{{{ ⇑! a' (length Γ) }}} equiv_len'_len' ↘ OEl' d{{{ ⇑! a' (length Γ) }}} equiv_len'_len' }} by mauto 4. *)
-(*     assert {{ Γ, IT' ⊢ OT ® OP d{{{ ⇑! a (length Γ) }}} equiv_len_len }}. *)
-(*     { *)
-(*       assert {{ Γ, IT ⊢ #0 : IT[Wk] ® ⇑! a (length Γ) ∈ IEl }} by (eapply var0_glu_elem; mauto 3). *)
-(*       assert {{ ⊢ Γ, IT' ≈ Γ, IT }} as -> by mauto. *)
-(*       assert {{ Γ, IT ⊢ OT[Wk,,#0] ≈ OT : Type@i }} as <- by (bulky_rewrite1; mauto 2). *)
-(*       mauto 4. *)
-(*     } *)
-(*     assert {{ Γ, IT' ⊢ OT' ® OP' d{{{ ⇑! a' (length Γ) }}} equiv_len'_len' }}. *)
-(*     { *)
-(*       assert {{ Γ, IT' ⊢ #0 : IT'[Wk] ® ⇑! a' (length Γ) ∈ IEl }} by (eapply var0_glu_elem; mauto 3). *)
-(*       assert {{ Γ, IT' ⊢ OT'[Wk,,#0] ® OP' d{{{ ⇑! a' (length Γ) }}} equiv_len'_len' }} by mauto 4. *)
-(*       assert {{ Γ, IT' ⊢ OT'[Wk,,#0] ≈ OT' : Type@i }} as <- by (bulky_rewrite1; mauto 2). *)
-(*       mauto 4. *)
-(*     } *)
-(*     mauto 3. *)
-(*   - match_by_head (per_bot b b') ltac:(fun H => specialize (H (length Γ)) as [V []]). *)
-(*     simpl in *. *)
-(*     destruct_conjs. *)
-(*     assert {{ Γ ⊢ A[Id] ≈ A : Type@i }} as <- by mauto 4. *)
-(*     assert {{ Γ ⊢ A'[Id] ≈ A' : Type@i }} as <- by mauto 3. *)
-(*     assert {{ Γ ⊢ A'[Id] ≈ V : Type@i }} as -> by mauto 4. *)
-(*     eapply wf_subtyp_refl'. *)
-(*     mauto 4. *)
-(* Qed. *)
-
-(* #[export] *)
-(* Hint Resolve glu_sort_elem_per_subtyp_typ_escape : mcpts. *)
-
-(* Lemma glu_sort_elem_per_subtyp_trm_if : forall {i a a' P P' El El' Γ A A' M m}, *)
-(*     {{ Sub a <: a' at i }} -> *)
-(*     {{ DG a ∈ glu_sort_elem i ↘ P ↘ El }} -> *)
-(*     {{ DG a' ∈ glu_sort_elem i ↘ P' ↘ El' }} -> *)
-(*     {{ Γ ⊢ A' ® P' }} -> *)
-(*     {{ Γ ⊢ M : A ® m ∈ El }} -> *)
-(*     {{ Γ ⊢ M : A' ® m ∈ El' }}. *)
-(* Proof. *)
-(*   intros * Hsubtyp Hglu Hglu' HA HA'. *)
-(*   assert {{ Γ ⊢ A ⊆ A' }} by (eapply glu_sort_elem_per_subtyp_typ_escape; only 4: eapply glu_sort_elem_trm_typ; mauto). *)
-(*   gen m M A' A. gen Γ. gen El' El P' P. *)
-(*   induction Hsubtyp using per_subtyp_ind; intros; subst; *)
-(*     saturate_refl_for per_sort_elem. *)
-(*   1-3,5: *)
-(*     invert_glu_sort_elem Hglu; *)
-(*   handle_functional_glu_sort_elem; *)
-(*   handle_per_sort_elem_irrel; *)
-(*   repeat invert_glu_rel1; *)
-(*   saturate_glu_by_per; *)
-(*   invert_glu_sort_elem Hglu'; *)
-(*   handle_functional_glu_sort_elem; *)
-(*   repeat invert_glu_rel1; *)
-(*   try solve [simpl in *; intuition mauto 3]. *)
-(*   - simpl in *. *)
-(*     destruct_conjs. *)
-(*     intuition mauto 3. *)
-(*     assert (exists P El, {{ DG m ∈ glu_sort_elem j ↘ P ↘ El }}) as [? [?]] by mauto 3. *)
-(*     do 2 eexists; split; mauto 3. *)
-(*     eapply glu_sort_elem_typ_cumu_ge; revgoals; mautosolve 3. *)
-(*   - rename A0 into A'. *)
-(*     rename IT0 into IT'. rename OT0 into OT'. *)
-(*     rename x into IP. rename x0 into IEl. *)
-(*     rename x1 into OP. rename x2 into OEl. *)
-(*     rename x3 into OP'. rename x4 into OEl'. *)
-(*     handle_per_sort_elem_irrel. *)
-(*     econstructor; mauto 3. *)
-(*     + enough {{ Sub Π a ρ B <: Π a' ρ' B' at i }} by (eapply per_elem_subtyping; try eassumption). *)
-(*       econstructor; mauto 3. *)
-(*     + intros. *)
-(*       assert {{ Γ ⊢w Id : Γ }} by mauto 3. *)
-(*       assert {{ Γ ⊢ IT ® IP }}. *)
-(*       { *)
-(*         assert {{ Γ ⊢ IT[Id] ® IP }} by mauto 3. *)
-(*         simpl in *. *)
-(*         autorewrite with mcpts in *; mauto 3. *)
-(*       } *)
-(*       assert {{ Γ ⊢ IT' ® IP }}. *)
-(*       { *)
-(*         assert {{ Γ ⊢ IT'[Id] ® IP }} by mauto 3. *)
-(*         simpl in *. *)
-(*         autorewrite with mcpts in *; mauto 3. *)
-(*       } *)
-(*       assert {{ Δ ⊢ IT'[σ] ≈ IT[σ] : Type@i }} by (symmetry; mauto 4 using glu_sort_elem_per_sort_typ_escape). *)
-(*       assert {{ Δ ⊢ N : IT'[σ] ® n ∈ IEl }} by (simpl; bulky_rewrite1; eassumption). *)
-(*       assert (exists mn : domain, {{ $| m & n |↘ mn }} /\ {{Δ ⊢ M[σ] N : OT'[σ,,N] ® mn ∈ OEl n equiv_n }}) by mauto 3. *)
-(*       destruct_conjs. *)
-(*       eexists; split; mauto 3. *)
-(*       match_by_head per_sort_elem ltac:(fun H => directed invert_per_sort_elem H). *)
-(*       destruct_rel_mod_eval. *)
-(*       handle_per_sort_elem_irrel. *)
-(*       match goal with *)
-(*       | _: {{ ⟦ B ⟧ ρ ↦ n ↘ ^?a }}, *)
-(*           _: {{ ⟦ B' ⟧ ρ' ↦ n ↘ ^?a' }} |- _ => *)
-(*           rename a into b; *)
-(*           rename a' into b' *)
-(*       end. *)
-(*       assert {{ DG b ∈ glu_sort_elem i ↘ OP n equiv_n ↘ OEl n equiv_n }} by mauto 3. *)
-(*       assert {{ DG b' ∈ glu_sort_elem i ↘ OP' n equiv_n ↘ OEl' n equiv_n }} by mauto 3. *)
-(*       assert {{ Δ ⊢ OT'[σ,,N] ® OP n equiv_n }} by (eapply glu_sort_elem_trm_typ; mauto 3). *)
-(*       assert {{ Sub b <: b' at i }} by mauto 3. *)
-(*       assert {{ Δ ⊢ OT'[σ,,N] ⊆ OT[σ,,N] }} by mauto 3. *)
-(*       intuition. *)
-(*   - match_by_head1 (per_bot b b') ltac:(fun H => destruct (H (length Γ)) as [V []]). *)
-(*     econstructor; mauto 3. *)
-(*     + econstructor; mauto 3. *)
-(*     + intros. *)
-(*       match_by_head1 (per_bot b b') ltac:(fun H => destruct (H (length Δ)) as [? []]). *)
-(*       functional_read_rewrite_clear. *)
-(*       assert {{ Δ ⊢ A[σ] ⊆ A'[σ] }} by mauto 3. *)
-(*       assert {{ Δ ⊢ M[σ] ≈ M' : A[σ] }} by mauto 3. *)
-(*       mauto 3. *)
-(*   - assert {{ Γ ⊢ A ® P }} by (eapply glu_sort_elem_trm_typ; eauto). *)
-(*     assert {{ Γ ⊢ A ≈ A' : Type@i }} by mauto 4. *)
-(*     rewrite H in *. *)
-(*     rewrite H4 in *. *)
-(*     handle_functional_glu_sort_elem. *)
-(*     trivial. *)
-(* Qed. *)
-
-(* Lemma glu_sort_elem_per_subtyp_trm_conv : forall {i j k a a' P P' El El' Γ A A' M m}, *)
-(*     {{ Sub a <: a' at i }} -> *)
-(*     {{ DG a ∈ glu_sort_elem j ↘ P ↘ El }} -> *)
-(*     {{ DG a' ∈ glu_sort_elem k ↘ P' ↘ El' }} -> *)
-(*     {{ Γ ⊢ A' ® P' }} -> *)
-(*     {{ Γ ⊢ M : A ® m ∈ El }} -> *)
-(*     {{ Γ ⊢ M : A' ® m ∈ El' }}. *)
-(* Proof. *)
-(*   intros. *)
-(*   assert {{ Sub a <: a' at (max i (max j k)) }} by mauto using per_subtyp_cumu_left. *)
-(*   assert (j <= max i (max j k)) by lia. *)
-(*   assert (exists P El, {{ DG a ∈ glu_sort_elem (max i (max j k)) ↘ P ↘ El }}) as [Ptop [Eltop]] by mauto using glu_sort_elem_cumu_ge. *)
-(*   assert (k <= max i (max j k)) by lia. *)
-(*   assert (exists P El, {{ DG a' ∈ glu_sort_elem (max i (max j k)) ↘ P ↘ El }}) as [Ptop' [Eltop']] by mauto using glu_sort_elem_cumu_ge. *)
-(*   assert {{ Γ ⊢ A' ® Ptop' }} by (eapply glu_sort_elem_typ_cumu_ge; mauto). *)
-(*   assert {{ Γ ⊢ M : A ® m ∈ Eltop }} by (eapply @glu_sort_elem_exp_cumu_ge with (i := j); mauto). *)
-(*   assert {{ Γ ⊢ M : A' ® m ∈ Eltop' }} by (eapply glu_sort_elem_per_subtyp_trm_if; mauto). *)
-(*   eapply glu_sort_elem_exp_lower; mauto. *)
-(* Qed. *)
-
-
-(** *** Lemmas for [glu_rel_typ_with_sub] and [glu_rel_exp_with_sub] *)
 
 Lemma mk_glu_rel_typ_with_sub' {P} (pred_P : PredicativeSig P) : forall {s Δ A σ ρ a},
     {{ ⟦ A ⟧ ρ ↘ a }} ->
@@ -743,6 +259,7 @@ Qed.
 #[export]
 Hint Resolve mk_glu_rel_typ_with_sub'' : mcpts.
 
+
 Lemma mk_glu_rel_exp_with_sub' {P} (pred_P : PredicativeSig P) : forall {s Δ A M σ ρ a m},
     {{ ⟦ A ⟧ ρ ↘ a }} ->
     {{ ⟦ M ⟧ ρ ↘ m }} ->
@@ -767,7 +284,7 @@ Lemma mk_glu_rel_exp_with_sub'' {P} (pred_P : PredicativeSig P) : forall {s Δ A
 Proof.
   intros * ? ? [] ?.
   assert (exists typ_rel exp_rel, {{ DG a ∈ glu_sort_elem pred_P s ↘ typ_rel ↘ exp_rel }}) as [? []] by mauto.
-  eapply mk_glu_rel_exp_with_sub'; mauto.
+  eapply mk_glu_rel_exp_with_sub'; mauto.  
 Qed.
 
 #[export]
@@ -775,11 +292,11 @@ Hint Resolve mk_glu_rel_exp_with_sub'' : mcpts.
 
 Lemma glu_rel_exp_with_sub_implies_glu_rel_exp_sub_with_typ {P} (pred_P : PredicativeSig P) : forall {s s' Δ A M σ Γ ρ},
     Ax P s s' ->
-      {{ Δ ⊢s σ : Γ }} ->
+    {{ Δ ⊢s σ : Γ }} ->
     glu_rel_exp_with_sub pred_P s Δ M A σ ρ ->
     glu_rel_exp_with_sub pred_P s' Δ A {{{ Sort@s }}} σ ρ.
 Proof.
-  intros * ax ? [].
+  intros * ? ? [].
   econstructor; mauto.
   assert {{ Δ ⊢ A[σ] : Sort@s }} by mauto using glu_sort_elem_trm_sort_lvl.
   repeat split; try do 2 eexists; mauto 3.
@@ -789,6 +306,7 @@ Qed.
 
 #[export]
 Hint Resolve glu_rel_exp_with_sub_implies_glu_rel_exp_sub_with_typ : mcpts.
+
 
 Lemma glu_rel_exp_with_sub_implies_glu_rel_typ_with_sub {P} (pred_P : PredicativeSig P) : forall {s Δ A s' σ ρ},
   glu_rel_exp_with_sub pred_P s Δ A {{{ Sort@s' }}} σ ρ ->
@@ -807,13 +325,14 @@ Qed.
 #[export]
 Hint Resolve glu_rel_exp_with_sub_implies_glu_rel_typ_with_sub : mcpts.
 
+
 Lemma glu_rel_typ_with_sub_implies_glu_rel_exp_with_sub {P} (pred_P : PredicativeSig P) : forall {Δ A s s' σ Γ ρ},
     Ax P s s' ->
     {{ Δ ⊢s σ : Γ }} ->
-  glu_rel_typ_with_sub pred_P s Δ A σ ρ ->
-  glu_rel_exp_with_sub pred_P s' Δ A {{{ Sort@s }}} σ ρ.
+    glu_rel_typ_with_sub pred_P s Δ A σ ρ ->
+    glu_rel_exp_with_sub pred_P s' Δ A {{{ Sort@s }}} σ ρ.
 Proof.
-  intros * ax ? [].
+  intros * ? ? [].
   simplify_evals.
   econstructor; mauto.
   assert {{ Δ ⊢ A[σ] : Sort@s }} by mauto 4 using glu_sort_elem_sort_lvl.
@@ -825,8 +344,8 @@ Hint Resolve glu_rel_typ_with_sub_implies_glu_rel_exp_with_sub : mcpts.
 
 (** *** Lemmas for [glu_ctx_env] *)
 
-Lemma glu_ctx_env_sub_resp_ctx_eq {P} (pred_P : PredicativeSig P) : forall {Γ Sb},
-    {{ EG Γ ∈ glu_ctx_env pred_P ↘ Sb }} ->
+Lemma glu_ctx_env_sub_resp_ctx_eq {P} (pred_P : PredicativeSig P) : forall {Γ sts Sb},
+    {{ EG Γ ∈ glu_ctx_env pred_P sts ↘ Sb }} ->
     forall {Δ Δ' σ ρ},
       {{ Δ ⊢s σ ® ρ ∈ Sb }} ->
       {{ ⊢ Δ ≈ Δ' }} ->
@@ -839,18 +358,18 @@ Proof.
 
   destruct_by_head (@cons_glu_sub_pred P).
   econstructor; mauto 4.
-  eapply glu_typ_unsorted_elem_trm_resp_ctx_eq; mauto.
+  rewrite <- Hctxeq; eassumption.
 Qed.
 
-Add Parametric Morphism {P} (pred_P : PredicativeSig P) Sb Γ (H : glu_ctx_env pred_P Sb Γ) : Sb
+Add Parametric Morphism {P} (pred_P : PredicativeSig P) sts Sb Γ (H : glu_ctx_env pred_P sts Sb Γ) : Sb
     with signature wf_ctx_eq ==> eq ==> eq ==> iff as glu_ctx_env_sub_morphism_iff1.
 Proof.
   intros.
   split; intros; eapply glu_ctx_env_sub_resp_ctx_eq; mauto.
 Qed.
 
-Lemma glu_ctx_env_sub_resp_sub_eq {P} (pred_P : PredicativeSig P) : forall {Γ Sb},
-    {{ EG Γ ∈ glu_ctx_env pred_P ↘ Sb }} ->
+Lemma glu_ctx_env_sub_resp_sub_eq {P} (pred_P : PredicativeSig P) : forall {sts Γ Sb},
+    {{ EG Γ ∈ glu_ctx_env pred_P sts ↘ Sb }} ->
     forall {Δ σ σ' ρ},
       {{ Δ ⊢s σ ® ρ ∈ Sb }} ->
       {{ Δ ⊢s σ ≈ σ' : Γ }} ->
@@ -865,24 +384,23 @@ Proof.
   destruct_by_head (@cons_glu_sub_pred P).
   econstructor; mauto 4.
   assert {{ Γ, A ⊢s Wk : Γ }} by mauto 3.
-  assert {{ Δ ⊢ A[Wk][σ] ≈ A[Wk][σ'] }} as <- by mauto 4.
-  assert {{ Δ ⊢ #0[σ] ≈ #0[σ'] : A[Wk][σ] }} as <- by mauto 3.  
+  assert {{ Δ ⊢ A[Wk][σ] ≈ A[Wk][σ'] : Sort@s }} as <- by mauto 4.
+  assert {{ Δ ⊢ #0[σ] ≈ #0[σ'] : A[Wk][σ] }} as <- by mauto 3.
   eassumption.
 Qed.
 
-Add Parametric Morphism {P} (pred_P : PredicativeSig P) Sb Γ (H : glu_ctx_env pred_P Sb Γ) Δ : (Sb Δ)
+Add Parametric Morphism {P} (pred_P : PredicativeSig P) sts Sb Γ (H : glu_ctx_env pred_P sts Sb Γ) Δ : (Sb Δ)
     with signature wf_sub_eq Δ Γ ==> eq ==> iff as glu_ctx_env_sub_morphism_iff2.
 Proof.
   split; intros; eapply glu_ctx_env_sub_resp_sub_eq; mauto.
 Qed.
 
-
-Lemma cons_glu_sub_pred_resp_wf_sub_eq {P} (pred_P : PredicativeSig P) : forall {Γ A Sb Δ σ σ' ρ},
-    {{ EG Γ ∈ glu_ctx_env pred_P ↘ Sb }} ->
-    {{ Γ ⊢ A }} ->
+Lemma cons_glu_sub_pred_resp_wf_sub_eq {P} (pred_P : PredicativeSig P) : forall {sts s Γ A Sb Δ σ σ' ρ},
+    {{ EG Γ ∈ glu_ctx_env pred_P sts ↘ Sb }} ->
+    {{ Γ ⊢ A : Sort@s }} ->
     {{ Δ ⊢s σ ≈ σ' : Γ, A }} ->
-    {{ Δ ⊢s σ ® ρ ∈ cons_glu_sub_pred pred_P Γ A Sb }} ->
-    {{ Δ ⊢s σ' ® ρ ∈ cons_glu_sub_pred pred_P Γ A Sb }}.
+    {{ Δ ⊢s σ ® ρ ∈ cons_glu_sub_pred pred_P s Γ A Sb }} ->
+    {{ Δ ⊢s σ' ® ρ ∈ cons_glu_sub_pred pred_P s Γ A Sb }}.
 Proof.
   intros * Hglu HA Heq Hσ.
   dependent destruction Hσ.
@@ -891,23 +409,19 @@ Proof.
   assert {{ Δ ⊢s Wk∘σ' : Γ }} by mauto 3.
   assert {{ Δ ⊢s Wk∘σ ≈ Wk∘σ' : Γ }} by mauto 3.
   econstructor; mauto 3.
-  - assert {{ Δ ⊢ A[Wk∘σ] ≈ A[Wk∘σ'] }} by mauto 3.
-    assert {{ Δ ⊢ A[Wk∘σ] ≈ A[Wk][σ] }} by mauto 4.
-    assert {{ Δ ⊢ A[Wk∘σ'] ≈ A[Wk][σ'] }} by mauto 4.
-    assert {{ Δ ⊢ A[Wk][σ] ≈ A[Wk][σ'] }} as <- by mauto 4.
+  - assert {{ Δ ⊢ A[Wk][σ] ≈ A[Wk][σ'] : Sort@s }} as <- by mauto.
     assert {{ Δ ⊢ #0[σ] ≈ #0[σ'] : A[Wk][σ] }} as <-; mauto 3.
   - assert {{ Δ ⊢s Wk∘σ ≈ Wk∘σ' : Γ }} as <-; eassumption.
 Qed.
 
-Add Parametric Morphism {P} (pred_P : PredicativeSig P) Γ A Sb Δ (Hglu : {{ EG Γ ∈ glu_ctx_env pred_P ↘ Sb }}) (HA : {{ Γ ⊢ A }}) : (cons_glu_sub_pred pred_P Γ A Sb Δ)
+Add Parametric Morphism {P} (pred_P : PredicativeSig P) sts s Γ A Sb Δ (Hglu : {{ EG Γ ∈ glu_ctx_env pred_P sts ↘ Sb }}) (HA : {{ Γ ⊢ A : Sort@s }}) : (cons_glu_sub_pred pred_P s Γ A Sb Δ)
     with signature wf_sub_eq Δ {{{ Γ, A }}} ==> eq ==> iff as cons_glu_sub_pred_morphism_iff.
 Proof.
   split; mauto using cons_glu_sub_pred_resp_wf_sub_eq.
 Qed.
 
-
-Lemma glu_ctx_env_per_env {P} (pred_P : PredicativeSig P) : forall {Γ Sb env_rel Δ σ ρ},
-    {{ EG Γ ∈ glu_ctx_env pred_P ↘ Sb }} ->
+Lemma glu_ctx_env_per_env {P} (pred_P : PredicativeSig P) : forall {sts Γ Sb env_rel Δ σ ρ},
+    {{ EG Γ ∈ glu_ctx_env pred_P sts ↘ Sb }} ->
     {{ EF Γ ≈ Γ ∈ per_ctx_env pred_P ↘ env_rel }} ->
     {{ Δ ⊢s σ ® ρ ∈ Sb }} ->
     {{ Dom ρ ≈ ρ ∈ env_rel }}.
@@ -919,39 +433,32 @@ Proof.
     apply_predicate_equivalence;
     handle_per_ctx_env_irrel;
     mauto 3.
-
-  (* rename i0 into j. *)
+  
   inversion_clear_by_head (@cons_glu_sub_pred P).
   assert {{ Dom ρ ↯ ≈ ρ ↯ ∈ tail_rel }} by intuition.
+  destruct_rel_typ.
   destruct_rel_typ_unsorted.
   handle_per_typ_elem_irrel.
-  handle_per_sort_elem_irrel.
-  
-  assert (exists typ_rel' exp_rel', {{ DG a ∈ glu_typ_unsorted_elem pred_P ↘ typ_rel' ↘ exp_rel' }}) as [? []] by mauto 3.
-  handle_functional_glu_typ_unsorted_elem P.
-  (* econstructor; mauto 2. *)
-  eexists; [eassumption | eassumption |].
+  assert (exists typ_rel' exp_rel', {{ DG a ∈ glu_sort_elem pred_P s ↘ typ_rel' ↘ exp_rel' }}) as [? []] by mauto 3.
 
-  eapply glu_typ_unsorted_elem_per_typ_elem; mauto.  
+  eexists; eauto.
+  handle_functional_glu_sort_elem P.
+  eapply glu_sort_elem_per_elem; mauto.
+  assert {{ Dom a ≈ a ∈ per_sort pred_P s }} by mauto 2.
+  unfold per_sort in H5.
+  destruct H5 as [].
+  mauto.
 Qed.
 
-
-Lemma glu_ctx_env_wf_ctx {P} (pred_P : PredicativeSig P) : forall {Γ Sb},
-    {{ EG Γ ∈ glu_ctx_env pred_P ↘ Sb }} ->
+Lemma glu_ctx_env_wf_ctx {P} (pred_P : PredicativeSig P) : forall {sts Γ Sb},
+    {{ EG Γ ∈ glu_ctx_env pred_P sts ↘ Sb }} ->
     {{ ⊢ Γ }}.
 Proof.
-  induction 1; intros; [| assert {{ Γ ⊢ A }} by mauto 3]; mauto.
+  induction 1; intros; mauto 3.
 Qed.
 
-Lemma glu_ctx_env_unsorted_wf_ctx {P} (pred_P : PredicativeSig P) : forall {Γ Sb},
-    {{ EG Γ ∈ glu_ctx_env_unsorted pred_P ↘ Sb }} ->
-    {{ ⊢ Γ }}.
-Proof.
-  induction 1; intros; [| assert {{ Γ ⊢ A }} by mauto 3]; mauto.
-Qed.
-
-Lemma glu_ctx_env_sub_escape {P} (pred_P : PredicativeSig P) : forall {Γ Sb},
-    {{ EG Γ ∈ glu_ctx_env pred_P ↘ Sb }} ->
+Lemma glu_ctx_env_sub_escape {P} (pred_P : PredicativeSig P) : forall {sts Γ Sb},
+    {{ EG Γ ∈ glu_ctx_env pred_P sts ↘ Sb }} ->
     forall Δ σ ρ,
       {{ Δ ⊢s σ ® ρ ∈ Sb }} ->
       {{ Δ ⊢s σ : Γ }}.
@@ -965,38 +472,22 @@ Qed.
 #[export]
 Hint Resolve glu_ctx_env_wf_ctx glu_ctx_env_sub_escape : mcpts.
 
-Lemma glu_ctx_env_per_ctx_env {P} (pred_P : PredicativeSig P) : forall {Γ Sb},
-    {{ EG Γ ∈ glu_ctx_env pred_P ↘ Sb }} ->
+Lemma glu_ctx_env_per_ctx_env {P} (pred_P : PredicativeSig P) : forall {sts Γ Sb},
+    {{ EG Γ ∈ glu_ctx_env pred_P sts ↘ Sb }} ->
     exists env_rel, {{ EF Γ ≈ Γ ∈ per_ctx_env pred_P ↘ env_rel }}.
 Proof.
   intros.
-  enough (valid_ctx pred_P Γ) by eassumption.
-  eapply completeness_fundamental_ctx.
-  eapply glu_ctx_env_wf_ctx; mauto 2.
+  enough {{ ⟪ pred_P ⟫ ⊨ Γ }} by eassumption.
+  mauto 3 using completeness_fundamental_ctx.
 Qed.
 
 #[export]
 Hint Resolve glu_ctx_env_per_ctx_env : mcpts.
 
 
-Lemma glu_ctx_env_unsorted_per_ctx_env {P} (pred_P : PredicativeSig P) : forall {Γ Sb},
-    {{ EG Γ ∈ glu_ctx_env_unsorted pred_P ↘ Sb }} ->
-    exists env_rel, {{ EF Γ ≈ Γ ∈ per_ctx_env pred_P ↘ env_rel }}.
-Proof.
-  intros.
-  enough (valid_ctx pred_P Γ) by eassumption.
-  eapply completeness_fundamental_ctx.
-  eapply glu_ctx_env_unsorted_wf_ctx; mauto 2.
-Qed.
-
-#[export]
-Hint Resolve glu_ctx_env_unsorted_per_ctx_env : mcpts.
-
-
-
-Lemma glu_ctx_env_resp_per_ctx_helper {P} (pred_P : PredicativeSig P) : forall {Γ Γ' Sb Sb'},
-    {{ EG Γ ∈ glu_ctx_env pred_P ↘ Sb }} ->
-    {{ EG Γ' ∈ glu_ctx_env pred_P ↘ Sb' }} ->
+Lemma glu_ctx_env_resp_per_ctx_helper {P} (pred_P : PredicativeSig P) : forall {sts Γ Γ' Sb Sb'},
+    {{ EG Γ ∈ glu_ctx_env pred_P sts ↘ Sb }} ->
+    {{ EG Γ' ∈ glu_ctx_env pred_P sts ↘ Sb' }} ->
     {{ ⊢ Γ ≈ Γ' }} ->
     (Sb -∙> Sb').
 Proof.
@@ -1012,75 +503,50 @@ Proof.
     handle_per_ctx_env_irrel;
     try firstorder.
 
-  
-  (* rename s0 into s'.   *)
   rename Γ0 into Γ'.
   rename A0 into A'.
   rename TSb0 into TSb'.
-  inversion HΓΓ' as [|? ? l]; subst.
+  
+  (* rename i0 into j. *)
+  (* rename Γ0 into Γ'. *)
+  (* rename A0 into A'. *)
+  (* rename TSb0 into TSb'. *)
+  (* rename i1 into k. *)
+
+  
+  inversion HΓΓ' as [|? ? l ? l']; subst.
   assert (TSb -∙> TSb') by intuition.
   intros Δ σ ρ [].
   saturate_refl_for (@per_ctx_env P).
-  assert {{ Dom ρ0 ↯ ≈ ρ0 ↯ ∈ tail_rel }}.
-  {
-    eapply glu_ctx_env_per_env; try eassumption.
-    transitivity Γ; [symmetry|]; eassumption.
-    eapply H14; eassumption.
-  }
+  assert {{ Dom ρ0 ↯ ≈ ρ0 ↯ ∈ tail_rel }}
+    by (eapply glu_ctx_env_per_env; [| | eassumption]; eassumption).
   assert {{ Δ0 ⊢s Wk∘σ0 ® ρ0 ↯ ∈ TSb' }} by intuition.
-  assert (glu_rel_typ_with_sub_unsorted pred_P Δ0 A' {{{ Wk∘σ0 }}} d{{{ ρ0 ↯ }}}) as [] by mauto 3.
-  
-  assert (rel_typ_unsorted pred_P A d{{{ ρ0 ↯ }}} A' d{{{ ρ0 ↯ }}} (head_rel _ _ H21)) by mauto 3.
+  assert (glu_rel_typ_with_sub pred_P s Δ0 A' {{{ Wk∘σ0 }}} d{{{ ρ0 ↯ }}}) as [] by mauto 3.
   destruct_rel_typ_unsorted.
-  handle_functional_glu_typ_unsorted_elem P.
-
+  handle_functional_glu_sort_elem P.
   rename a0 into a'.
-  (* rename El0 into El'. *)
-  rename P0 into P'.
-
-  assert {{ Δ0 ⊢ A'[Wk∘σ0] }} by (eapply glu_typ_unsorted_elem_sort_lvl; mauto 3).
-  assert {{ Δ0 ⊢ A'[Wk∘σ0] ≈ A'[Wk][σ0] }} by mauto 4.
-  assert {{ Δ0 ⊢ A'[Wk][σ0] }} by (gen_presup H3; eassumption).
-  
+  rename El0 into exp_rel'.
+  rename P0 into typ_rel'.
   econstructor; mauto 4.
 
-  assert {{ Δ0 ⊢ #0[σ0] : A[Wk][σ0] ® m ∈ El }}.
-  {
-    admit. (* need glu_typ_unsorted_elem_exp_conv to solve this goal *)
-    (* eapply glu_sort_elem_exp_conv; mauto 3. *)
-  }
-  
-  (* assert {{ Δ0 ⊢ A[Wk][σ0] : Sort@s }} by (eapply glu_sort_elem_trm_sort_lvl; mauto 3). *)
-  
+  assert (per_typ pred_P a a') by mauto 3.
+  assert ((typ_rel' <∙> P1) /\ (El <∙> exp_rel')) by (eapply glu_sort_elem_per_typ_iff; mauto 2).
+  destruct_conjs.
+  eapply H33.
 
-  
-  assert (exists Pmax Elmax, {{ DG a ∈ glu_sort_elem (max i l) ↘ Pmax ↘ Elmax }}) as [Pmax [Elmax]]
-      by mauto using glu_sort_elem_cumu_max_left.
-  assert (i <= max i l) by lia.
-
-  
-  
-  assert {{ Δ0 ⊢ #0[σ0] : A[Wk][σ0] ® m ∈ El' }}.
-  {
-    eapply glu_sort_elem_exp_conv with (exp_rel := El); mauto.
-    
-    assert {{ Γ, A ⊢s Wk : Γ }} by mauto 3.
-    assert {{ Δ0 ⊢ A[Wk][σ0] ≈ A'[Wk][σ0] }} by mauto 3.
-    
-    
-    enough (El' Δ0 {{{ A[Wk][σ0] }}} {{{ #0[σ0] }}} m) by (eapply .
-    assert {{ Δ0 ⊢ A[Wk][σ0] ≈ A'[Wk][σ0] }} as <- by mauto 3.
-    eapply glu_sort_elem_exp_cumu_ge; mauto 3.
-  }
-  eapply glu_sort_elem_exp_conv; [eexists | | | |]; intuition.
-  autorewrite with mcpts.
-  eassumption.
-Admitted.
+  enough {{ Δ0 ⊢ A[Wk][σ0] ≈ A'[Wk][σ0] : Sort@s }} by (eapply glu_sort_elem_trm_resp_typ_exp_eq; mauto 2).
+  assert (typ_rel' Δ0 {{{ A[Wk][σ0] }}}) by (eapply glu_sort_elem_trm_typ; mauto 2).
+  apply_predicate_equivalence.
+  assert {{ Δ0 ⊢ A[Wk][σ0] ≈ A'[Wk∘σ0] : Sort@s }} by mauto 2.
+  transitivity {{{ A'[Wk∘σ0] }}}; mauto 2.
+  eapply exp_eq_sub_compose_typ_sort; mauto 2.
+  econstructor; mauto 3.
+Qed.
 
 
-Corollary functional_glu_ctx_env {P} (pred_P : PredicativeSig P) : forall {Γ Sb Sb'},
-    {{ EG Γ ∈ glu_ctx_env pred_P ↘ Sb }} ->
-    {{ EG Γ ∈ glu_ctx_env pred_P ↘ Sb' }} ->
+Corollary functional_glu_ctx_env {P} (pred_P : PredicativeSig P) : forall {sts Γ Sb Sb'},
+    {{ EG Γ ∈ glu_ctx_env pred_P sts ↘ Sb }} ->
+    {{ EG Γ ∈ glu_ctx_env pred_P sts ↘ Sb' }} ->
     (Sb <∙> Sb').
 Proof.
   intros.
@@ -1088,11 +554,12 @@ Proof.
   split; eapply glu_ctx_env_resp_per_ctx_helper; eassumption.
 Qed.
 
+
 Ltac apply_functional_glu_ctx_env1 :=
   let tactic_error o1 o2 := fail 2 "functional_glu_ctx_env biconditional between" o1 "and" o2 "cannot be solved" in
   match goal with
-  | H1 : {{ EG ^?Γ ∈ glu_ctx_env ↘ ?Sb1 }},
-      H2 : {{ EG ^?Γ ∈ glu_ctx_env ↘ ?Sb2 }} |- _ =>
+  | H1 : {{ EG ^?Γ ∈ glu_ctx_env ?pred_P ?sts ↘ ?Sb1 }},
+      H2 : {{ EG ^?Γ ∈ glu_ctx_env ?pred_P ?sts ↘ ?Sb2 }} |- _ =>
       assert_fails (unify Sb1 Sb2);
       match goal with
       | H : Sb1 <∙> Sb2 |- _ => fail 1
@@ -1103,81 +570,58 @@ Ltac apply_functional_glu_ctx_env1 :=
 Ltac apply_functional_glu_ctx_env :=
   repeat apply_functional_glu_ctx_env1.
 
-Ltac handle_functional_glu_ctx_env :=
+Ltac handle_functional_glu_ctx_env P :=
   functional_eval_rewrite_clear;
-  fold glu_typ_pred in *;
-  fold glu_exp_pred in *;
+  fold (glu_typ_pred P) in *;
+  fold (glu_exp_pred P) in *;
   apply_functional_glu_ctx_env;
   apply_predicate_equivalence;
   clear_dups.
 
-Lemma glu_ctx_env_cons_clean_inversion : forall {Γ TSb A Sb},
-  {{ EG Γ ∈ glu_ctx_env ↘ TSb }} ->
-  {{ EG Γ, A ∈ glu_ctx_env ↘ Sb }} ->
-  exists i,
-    {{ Γ ⊢ A : Type@i }} /\
+Lemma glu_ctx_env_cons_clean_inversion {P} (pred_P : PredicativeSig P) : forall {sts s Γ TSb A Sb},
+  {{ EG Γ ∈ glu_ctx_env pred_P sts ↘ TSb }} ->
+  {{ EG Γ, A ∈ glu_ctx_env pred_P (cons s sts) ↘ Sb }} ->
+  {{ Γ ⊢ A : Sort@s }} /\
       (forall Δ σ ρ,
           {{ Δ ⊢s σ ® ρ ∈ TSb }} ->
-          glu_rel_typ_with_sub i Δ A σ ρ) /\
-      (Sb <∙> cons_glu_sub_pred i Γ A TSb).
+          glu_rel_typ_with_sub pred_P s Δ A σ ρ) /\
+      (Sb <∙> cons_glu_sub_pred pred_P s Γ A TSb).
 Proof.
   intros.
   simpl in *.
-  match_by_head glu_ctx_env progressive_invert.
+  match_by_head (@glu_ctx_env P) progressive_invert.
   apply_functional_glu_ctx_env.
-  eexists; intuition.
-  assert (Sb <∙> cons_glu_sub_pred i Γ A TSb0) as -> by eassumption.
+  intuition.
+  rewrite -> H3.
+  (* assert (Sb <∙> cons_glu_sub_pred pred_P s Γ A TSb0) as -> by eassumption. *)
   intros Δ σ ρ.
   split; intros [];
     econstructor; intuition.
 Qed.
 
 Ltac invert_glu_ctx_env H :=
-  (unshelve eapply (glu_ctx_env_cons_clean_inversion _) in H; shelve_unifiable; [eassumption |];
+  (unshelve eapply (glu_ctx_env_cons_clean_inversion _ _ _ _) in H; shelve_unifiable; [eassumption |];
    destruct H as [? [? []]])
   + dependent destruction H.
 
-Lemma glu_ctx_env_subtyp_sub_if : forall Γ Γ' Sb Sb' Δ σ ρ,
-    {{ ⊢ Γ ⊆ Γ' }} ->
-    {{ EG Γ ∈ glu_ctx_env ↘ Sb }} ->
-    {{ EG Γ' ∈ glu_ctx_env ↘ Sb' }} ->
+
+Lemma glu_ctx_env_eqtyp_sub_if {P} (pred_P : PredicativeSig P) : forall sts Γ Γ' Sb Sb' Δ σ ρ,
+    {{ ⊢ Γ ≈ Γ' }} ->
+    {{ EG Γ ∈ glu_ctx_env pred_P sts ↘ Sb }} ->
+    {{ EG Γ' ∈ glu_ctx_env pred_P sts ↘ Sb' }} ->
     {{ Δ ⊢s σ ® ρ ∈ Sb }} ->
     {{ Δ ⊢s σ ® ρ ∈ Sb' }}.
 Proof.
-  intros * Hsubtyp Hglu Hglu'.
-  gen ρ σ Δ. gen Sb' Sb.
-  induction Hsubtyp; intros;
-    invert_glu_ctx_env Hglu;
-    invert_glu_ctx_env Hglu';
-    handle_functional_glu_ctx_env;
-    eauto.
-
-  rename Δ into Γ'.
-  rename i0 into j.
-  rename i1 into k.
-  rename TSb0 into TSb'.
-  destruct_by_head cons_glu_sub_pred.
-  assert (glu_rel_typ_with_sub k Δ A' {{{ Wk∘σ }}} d{{{ ρ ↯ }}}) as [] by intuition.
-  rename a0 into a'.
-  rename P0 into P'.
-  rename El0 into El'.
-  assert (exists tail_rel, {{ EF Γ ≈ Γ ∈ per_ctx_env ↘ tail_rel }}) as [tail_rel] by mauto 3 using glu_ctx_env_per_ctx_env.
-  assert {{ Dom ρ ↯ ≈ ρ ↯ ∈ tail_rel }} by (eapply glu_ctx_env_per_env; revgoals; eassumption).
-  assert {{ ⊢ Γ, A ⊆ Γ', A' }} by mauto 3.
-  econstructor; mauto; intuition.
-  assert {{ Γ ⊨ A ⊆ A' }} as [] by mauto 3 using completeness_fundamental_subtyp.
-  destruct_conjs.
-  handle_per_ctx_env_irrel.
-  (on_all_hyp_rev: destruct_rel_by_assumption tail_rel).
-  destruct_by_head rel_exp.
-  handle_functional_glu_ctx_env.
-  eapply glu_sort_elem_per_subtyp_trm_conv; mauto 3.
-  autorewrite with mcpts.
+  intros * HΓΓ' HgluΓ HgluΓ'.
+  assert (Sb -∙> Sb') by (eapply glu_ctx_env_resp_per_ctx_helper; mauto 2).
+  intros.
+  eapply H.
   eassumption.
 Qed.
 
-Lemma glu_ctx_env_sub_monotone : forall Γ Sb,
-    {{ EG Γ ∈ glu_ctx_env ↘ Sb }} ->
+
+Lemma glu_ctx_env_sub_monotone {P} (pred_P : PredicativeSig P) : forall sts Γ Sb,
+    {{ EG Γ ∈ glu_ctx_env pred_P sts ↘ Sb }} ->
     forall Δ' σ Δ τ ρ,
       {{ Δ ⊢s τ ® ρ ∈ Sb }} ->
       {{ Δ' ⊢w σ : Δ }} ->
@@ -1188,14 +632,19 @@ Proof.
     simpl in *;
     mauto 3.
 
-  destruct_by_head cons_glu_sub_pred.
+  destruct_by_head (@cons_glu_sub_pred P).
   econstructor; mauto 3.
-  - assert {{ Δ' ⊢ #0[σ0][σ] : A[Wk][σ0][σ] ® ^(ρ 0) ∈ El }} by (eapply glu_sort_elem_exp_monotone; mauto 3).
+  - assert {{ Δ' ⊢ #0[σ0][σ] : A[Wk][σ0][σ] ® m ∈ El }} by (eapply glu_sort_elem_exp_monotone; mauto 3).
     assert {{ Γ, A ⊢ #0 : A[Wk] }} by mauto 3.
     assert {{ Γ, A ⊢s Wk : Γ }} by mauto 3.
     assert {{ Δ' ⊢ #0[σ0∘σ] ≈ #0[σ0][σ] : A[Wk][σ0∘σ] }} as -> by mauto 3.
     assert {{ Δ' ⊢s σ : Δ }} by mauto 3.
-    assert {{ Δ' ⊢ A[Wk][σ0][σ] ≈ A[Wk][σ0∘σ] : Type@i }} as <- by mauto 3.
+    assert {{ Δ' ⊢ A[Wk][σ0][σ] ≈ A[Wk][σ0∘σ] : Sort@s }} as <-.
+    {
+      symmetry.
+      eapply exp_eq_sub_compose_typ_sort; mauto 2.
+      eapply eq_exp_sub_typ; mauto 2.
+    }
     eassumption.
   - assert {{ Δ' ⊢s σ : Δ }} by mauto 3.
     assert {{ Γ, A ⊢s Wk : Γ }} by mauto 3.
@@ -1203,14 +652,14 @@ Proof.
     mauto 3.
 Qed.
 
-Lemma cons_glu_sub_pred_helper : forall {Γ Sb Δ σ ρ A a i P El M c},
-    {{ EG Γ ∈ glu_ctx_env ↘ Sb }} ->
+Lemma cons_glu_sub_pred_helper {P} (pred_P : PredicativeSig P) : forall {sts Γ Sb Δ σ ρ A a s P El M c},
+    {{ EG Γ ∈ glu_ctx_env pred_P sts ↘ Sb }} ->
     {{ Δ ⊢s σ ® ρ ∈ Sb }} ->
-    {{ Γ ⊢ A : Type@i }} ->
+    {{ Γ ⊢ A : Sort@s }} ->
     {{ ⟦ A ⟧ ρ ↘ a }} ->
-    {{ DG a ∈ glu_sort_elem i ↘ P ↘ El }} ->
+    {{ DG a ∈ glu_sort_elem pred_P s ↘ P ↘ El }} ->
     {{ Δ ⊢ M : A[σ] ® c ∈ El }} ->
-    {{ Δ ⊢s σ,,M ® ρ ↦ c ∈ cons_glu_sub_pred i Γ A Sb }}.
+    {{ Δ ⊢s σ,,M ® ρ ↦ c ∈ cons_glu_sub_pred pred_P s Γ A Sb }}.
 Proof.
   intros.
   assert {{ Δ ⊢s σ : Γ }} by mauto 2.
@@ -1219,15 +668,28 @@ Proof.
   econstructor; mauto 3;
     autorewrite with mcpts; mauto 3.
 
-  assert {{ Δ ⊢ #0[σ,,M] ≈ M : A[σ] }} as ->; mauto 2.
+  assert {{ Δ ⊢ #0[σ,,M] ≈ M : A[σ] }}; mauto 2.
+  assert {{ Δ ⊢ A[Wk][σ,,M] ≈ A[σ] : Sort@s }}.
+  {
+    transitivity {{{ A[Wk∘(σ,,M)] }}}; mauto 2.
+    - symmetry; eapply exp_eq_sub_compose_typ_sort; mauto 2.
+      econstructor; mauto 2.
+    - eapply eq_exp_eq_sub_typ; mauto 2.
+      econstructor; mauto 2.
+      econstructor; mauto 2.
+  }
+  enough (El Δ {{{ A[σ] }}} {{{ #0[σ,,M] }}} c) by (eapply glu_sort_elem_trm_resp_typ_exp_eq; mauto 3).  
+  enough (El Δ {{{ A[σ] }}} M c) by (eapply glu_sort_elem_trm_resp_exp_eq; mauto 4).
+  mauto.
 Qed.
 
 #[export]
 Hint Resolve cons_glu_sub_pred_helper : mcpts.
 
-Lemma initial_env_glu_rel_exp : forall {Γ ρ Sb},
+
+Lemma initial_env_glu_rel_exp {P} (pred_P : PredicativeSig P) : forall {sts Γ ρ Sb},
     initial_env Γ ρ ->
-    {{ EG Γ ∈ glu_ctx_env ↘ Sb }} ->
+    {{ EG Γ ∈ glu_ctx_env pred_P sts ↘ Sb }} ->
     {{ Γ ⊢s Id ® ρ ∈ Sb }}.
 Proof.
   intros * Hinit HΓ.
@@ -1237,25 +699,29 @@ Proof.
     apply_predicate_equivalence;
     try solve [econstructor; mauto].
 
-  assert (glu_rel_typ_with_sub i Γ A {{{ Id }}} ρ) as [] by mauto.
+  rename ρ0 into ρ.
+  assert (glu_rel_typ_with_sub pred_P s Γ A {{{ Id }}} ρ) as [] by mauto.
+  rename P0 into typ_rel.
+  
   functional_eval_rewrite_clear.
   econstructor; mauto.
   - match goal with
-    | H: P Γ {{{ A[Id] }}} |- _ =>
+    | H: typ_rel Γ {{{ A[Id] }}} |- _ =>
         bulky_rewrite_in H
     end.
     eapply realize_glu_elem_bot; mauto.
     assert {{ ⊢ Γ }} by mauto 3.
     assert {{ Γ, A ⊢s Wk : Γ }} by mauto 4.
-    assert {{ Γ, A ⊢ A[Wk] : Type@i }} by mauto 4.
-    assert {{ Γ, A ⊢ A[Wk] ≈ A[Wk][Id] : Type@i }} as <- by mauto 3.
+    assert {{ Γ, A ⊢ A[Wk] : Sort@s }} by mauto 4.
+    assert {{ Γ, A ⊢ A[Wk] ≈ A[Wk][Id] : Sort@s }} as <- by mauto 3.
     assert {{ Γ, A ⊢ #0 ≈ #0[Id] : A[Wk] }} as <- by mauto.
     eapply var_glu_elem_bot; mauto.
   - assert {{ Γ, A ⊢s Wk : Γ }} by mauto 4.
     assert {{ Γ, A ⊢s Wk∘Id : Γ }} by mauto 4.
-    assert {{ Γ, A ⊢s Id∘Wk ≈ Wk∘Id : Γ }} as <- by (transitivity {{{ Wk }}}; mauto 3).
+    assert {{ Γ, A ⊢s Id∘Wk ≈ Wk∘Id : Γ }} as <- by (transitivity (@a_weaken P); mauto 3).
     eapply glu_ctx_env_sub_monotone; mauto 4.
 Qed.
+
 
 (** *** Tactics for [glu_rel_*] *)
 
@@ -1273,9 +739,9 @@ Ltac destruct_glu_rel_by_assumption sub_glu_rel H :=
 Ltac destruct_glu_rel_exp_with_sub :=
   repeat
     match goal with
-    | H : (forall Δ σ ρ, {{ Δ ⊢s σ ® ρ ∈ ?sub_glu_rel }} -> glu_rel_exp_with_sub _ _ _ _ _ _) |- _ =>
+    | H : (forall Δ σ ρ, {{ Δ ⊢s σ ® ρ ∈ ?sub_glu_rel }} -> glu_rel_exp_with_sub _ _ _ _ _ _ _) |- _ =>
         destruct_glu_rel_by_assumption sub_glu_rel H; fail_if_dup; mark H
-    | H : glu_rel_exp_with_sub _ _ _ _ _ _ |- _ =>
+    | H : glu_rel_exp_with_sub _ _ _ _ _ _ _ |- _ =>
         dependent destruction H
     end;
   unmark_all.
@@ -1283,9 +749,9 @@ Ltac destruct_glu_rel_exp_with_sub :=
 Ltac destruct_glu_rel_sub_with_sub :=
   repeat
     match goal with
-    | H : (forall Δ σ ρ, {{ Δ ⊢s σ ® ρ ∈ ?sub_glu_rel }} -> glu_rel_sub_with_sub _ _ _ _ _) |- _ =>
+    | H : (forall Δ σ ρ, {{ Δ ⊢s σ ® ρ ∈ ?sub_glu_rel }} -> glu_rel_sub_with_sub _ _ _ _ _ _) |- _ =>
         destruct_glu_rel_by_assumption sub_glu_rel H; fail_if_dup; mark H
-    | H : glu_rel_exp_with_sub _ _ _ _ _ _ |- _ =>
+    | H : glu_rel_exp_with_sub _ _ _ _ _ _ _ |- _ =>
         dependent destruction H
     end;
   unmark_all.
@@ -1293,68 +759,76 @@ Ltac destruct_glu_rel_sub_with_sub :=
 Ltac destruct_glu_rel_typ_with_sub :=
   repeat
     match goal with
-    | H : (forall Δ σ ρ, {{ Δ ⊢s σ ® ρ ∈ ?sub_glu_rel }} -> glu_rel_typ_with_sub _ _ _ _ _) |- _ =>
+    | H : (forall Δ σ ρ, {{ Δ ⊢s σ ® ρ ∈ ?sub_glu_rel }} -> glu_rel_typ_with_sub _ _ _ _ _ _) |- _ =>
         destruct_glu_rel_by_assumption sub_glu_rel H; fail_if_dup; mark H
-    | H : glu_rel_exp_with_sub _ _ _ _ _ _ |- _ =>
+    | H : glu_rel_exp_with_sub _ _ _ _ _ _ _ |- _ =>
         dependent destruction H
     end;
   unmark_all.
 
+
 (** *** Lemmas about [glu_rel_exp] *)
 
-Lemma glu_rel_exp_clean_inversion1 : forall {Γ Sb M A},
-    {{ EG Γ ∈ glu_ctx_env ↘ Sb }} ->
-    {{ Γ ⊩ M : A }} ->
-    exists i,
+Lemma glu_rel_exp_clean_inversion1 {P} (pred_P : PredicativeSig P) : forall {sts Γ Sb M A},
+    {{ EG Γ ∈ glu_ctx_env pred_P sts ↘ Sb }} ->
+    glu_rel_exp pred_P Γ sts M A ->
+    (* {{ ⟪ pred_P ⟫ Γ : sts ⊩ M : A }} -> *)
+    exists s,
     forall Δ σ ρ,
       {{ Δ ⊢s σ ® ρ ∈ Sb }} ->
-      glu_rel_exp_with_sub i Δ M A σ ρ.
+      glu_rel_exp_with_sub pred_P s Δ M A σ ρ.
 Proof.
   intros * ? [].
   destruct_conjs.
   eexists; intros.
-  handle_functional_glu_ctx_env.
+  handle_functional_glu_ctx_env P.
   mauto.
 Qed.
 
-Lemma glu_rel_exp_clean_inversion2 : forall {i Γ Sb M A},
-    {{ EG Γ ∈ glu_ctx_env ↘ Sb }} ->
-    {{ Γ ⊩ A : Type@i }} ->
-    {{ Γ ⊩ M : A }} ->
-    glu_rel_exp_resp_sub_env i Sb M A.
+Lemma glu_rel_exp_clean_inversion2 {P} (pred_P : PredicativeSig P) : forall {sts s Γ Sb M A},
+    {{ EG Γ ∈ glu_ctx_env pred_P sts ↘ Sb }} ->
+    glu_rel_exp pred_P Γ sts A {{{ Sort@s }}} ->
+    (* {{ ⟪ pred_P ⟫ Γ :: sts ⊩ A : Sort@s }} -> *)
+    glu_rel_exp pred_P Γ sts M A ->
+    (* {{ ⟪ pred_P ⟫ Γ :: sts ⊩ M : A }} -> *)
+    glu_rel_exp_resp_sub_env pred_P s Sb M A.
 Proof.
   simpl.
   intros * ? HA HM.
   eapply glu_rel_exp_clean_inversion1 in HA; [| eassumption].
   eapply glu_rel_exp_clean_inversion1 in HM; [| eassumption].
-  destruct_conjs.
+  destruct HA as [s0 ?].
+  destruct HM as [s1 ?].
   intros.
   destruct_glu_rel_exp_with_sub.
   simplify_evals.
-  match_by_head glu_sort_elem ltac:(fun H => directed invert_glu_sort_elem H).
+  match_by_head (@glu_sort_elem P) ltac:(fun H => directed invert_glu_sort_elem H).
   apply_predicate_equivalence.
   unfold sort_glu_exp_pred' in *.
+  unfold glu_sort_typ_rec in *.
   destruct_conjs.
   econstructor; mauto 3.
   eapply glu_sort_elem_exp_conv; revgoals; mauto 3.
 Qed.
 
+
 #[global]
 Ltac invert_glu_rel_exp H :=
-  (unshelve eapply (glu_rel_exp_clean_inversion2 _ _) in H; shelve_unifiable; [eassumption | eassumption |];
+  (unshelve eapply (glu_rel_exp_clean_inversion2 _ _ _ _ _) in H; shelve_unifiable; [eassumption | eassumption |];
    simpl in H)
-  + (unshelve eapply (glu_rel_exp_clean_inversion1 _) in H; shelve_unifiable; [eassumption |];
+  + (unshelve eapply (glu_rel_exp_clean_inversion1 _ _ _ _) in H; shelve_unifiable; [eassumption |];
      destruct H as [])
   + (inversion H as [? [? [? ?]]]; subst).
 
 
-Lemma glu_rel_exp_to_wf_exp : forall {Γ A M},
-    {{ Γ ⊩ M : A }} ->
+Lemma glu_rel_exp_to_wf_exp {P} (pred_P : PredicativeSig P) : forall {sts Γ A M},
+    glu_rel_exp pred_P Γ sts M A  ->
+    (* {{ ⟪ pred_P ⟫ Γ :: sts ⊩ M : A }} -> *)
     {{ Γ ⊢ M : A }}.
 Proof.
   intros * [Sb].
   destruct_conjs.
-  assert (exists env_rel, {{ EF Γ ≈ Γ ∈ per_ctx_env ↘ env_rel }}) as [env_rel] by mauto 3.
+  assert (exists env_rel, {{ EF Γ ≈ Γ ∈ per_ctx_env pred_P ↘ env_rel }}) as [env_rel] by mauto 3.
   assert (exists ρ ρ', initial_env Γ ρ /\ initial_env Γ ρ' /\ {{ Dom ρ ≈ ρ' ∈ env_rel }}) as [ρ] by mauto using per_ctx_then_per_env_initial_env.
   destruct_conjs.
   functional_initial_env_rewrite_clear.
@@ -1368,68 +842,72 @@ Hint Resolve glu_rel_exp_to_wf_exp : mcpts.
 
 (** *** Lemmas about [glu_rel_sub] *)
 
-Lemma glu_rel_sub_clean_inversion1 : forall {Γ Sb τ Γ'},
-    {{ EG Γ ∈ glu_ctx_env ↘ Sb }} ->
-    {{ Γ ⊩s τ : Γ' }} ->
-    exists Sb' : glu_sub_pred,
-      glu_ctx_env Sb' Γ' /\ (forall (Δ : ctx) (σ : sub) (ρ : env), Sb Δ σ ρ -> glu_rel_sub_with_sub Δ τ Sb' σ ρ).
+Lemma glu_rel_sub_clean_inversion1 {P} (pred_P : PredicativeSig P) : forall {sts sts' Γ Sb τ Γ'},
+    {{ EG Γ ∈ glu_ctx_env pred_P sts ↘ Sb }} ->
+    glu_rel_sub pred_P Γ sts τ Γ' sts' ->
+    (* {{ ⟪ pred_P ⟫ Γ :: sts ⊩s τ : Γ' }} -> *)
+    exists Sb' : glu_sub_pred P,
+      glu_ctx_env pred_P sts' Sb' Γ' /\ (forall (Δ : ctx P) (σ : sub P) (ρ : env P), Sb Δ σ ρ -> glu_rel_sub_with_sub pred_P Δ τ Sb' σ ρ).
 Proof.
   intros * ? [? []].
   destruct_conjs.
-  handle_functional_glu_ctx_env.
+  handle_functional_glu_ctx_env P.
   eexists; split; mauto 3.
   intros.
-  rewrite_predicate_equivalence_right.
+  rewrite_predicate_equivalence_left.
   mauto 3.
 Qed.
 
-Lemma glu_rel_sub_clean_inversion2 : forall {Γ τ Γ' Sb'},
-    {{ EG Γ' ∈ glu_ctx_env ↘ Sb' }} ->
-    {{ Γ ⊩s τ : Γ' }} ->
-    exists Sb : glu_sub_pred,
-      glu_ctx_env Sb Γ /\ (forall (Δ : ctx) (σ : sub) (ρ : env), Sb Δ σ ρ -> glu_rel_sub_with_sub Δ τ Sb' σ ρ).
+Lemma glu_rel_sub_clean_inversion2 {P} (pred_P : PredicativeSig P) : forall {sts sts' Γ τ Γ' Sb'},
+    {{ EG Γ' ∈ glu_ctx_env pred_P sts' ↘ Sb' }} ->
+    glu_rel_sub pred_P Γ sts τ Γ' sts' ->
+    (* {{ Γ ⊩s τ : Γ' }} -> *)
+    exists Sb : glu_sub_pred P,
+      glu_ctx_env pred_P sts Sb Γ /\ (forall (Δ : ctx P) (σ : sub P) (ρ : env P), Sb Δ σ ρ -> glu_rel_sub_with_sub pred_P Δ τ Sb' σ ρ).
 Proof.
   intros * ? [? [Sb'0]].
   destruct_conjs.
-  handle_functional_glu_ctx_env.
+  handle_functional_glu_ctx_env P.  
   eexists; split; mauto 3.
   intros.
-  assert (glu_rel_sub_with_sub Δ τ Sb'0 σ ρ) as [] by mauto 3.
+  assert (glu_rel_sub_with_sub pred_P Δ τ Sb'0 σ ρ) as [] by mauto 3.
   econstructor; mauto 3.
-  rewrite_predicate_equivalence_right.
+  rewrite_predicate_equivalence_left.
   mauto 3.
 Qed.
 
-Lemma glu_rel_sub_clean_inversion3 : forall {Γ Sb τ Γ' Sb'},
-    {{ EG Γ ∈ glu_ctx_env ↘ Sb }} ->
-    {{ EG Γ' ∈ glu_ctx_env ↘ Sb' }} ->
-    {{ Γ ⊩s τ : Γ' }} ->
-    glu_rel_sub_resp_sub_env Sb Sb' τ.
+Lemma glu_rel_sub_clean_inversion3 {P} (pred_P : PredicativeSig P) : forall {sts sts' Γ Sb τ Γ' Sb'},
+    {{ EG Γ ∈ glu_ctx_env pred_P sts ↘ Sb }} ->
+    {{ EG Γ' ∈ glu_ctx_env pred_P sts' ↘ Sb' }} ->
+    glu_rel_sub pred_P Γ sts τ Γ' sts' ->
+    (* {{ Γ ⊩s τ : Γ' }} -> *)
+    glu_rel_sub_resp_sub_env pred_P Sb Sb' τ.
 Proof.
   simpl. intros * ? ? Hglu.
   eapply glu_rel_sub_clean_inversion2 in Hglu; [| eassumption].
   destruct_conjs.
-  handle_functional_glu_ctx_env.
+  handle_functional_glu_ctx_env P.
   intros.
   rewrite_predicate_equivalence_right.
   mauto 3.
 Qed.
 
 Ltac invert_glu_rel_sub H :=
-  (unshelve eapply (glu_rel_sub_clean_inversion3 _ _) in H; shelve_unifiable; [eassumption | eassumption |])
-  + (unshelve eapply (glu_rel_sub_clean_inversion2 _) in H; shelve_unifiable; [eassumption |];
+  (unshelve eapply (glu_rel_sub_clean_inversion3 _ _ _ _ _ _) in H; shelve_unifiable; [eassumption | eassumption |])
+  + (unshelve eapply (glu_rel_sub_clean_inversion2 _ _ _ _ _) in H; shelve_unifiable; [eassumption |];
      destruct H as [? []])
-  + (unshelve eapply (glu_rel_sub_clean_inversion1 _) in H; shelve_unifiable; [eassumption |];
+  + (unshelve eapply (glu_rel_sub_clean_inversion1 _ _ _ _ _) in H; shelve_unifiable; [eassumption |];
      destruct H as [? []])
   + (inversion H; subst).
 
-Lemma glu_rel_sub_wf_sub : forall {Γ σ Δ},
-    {{ Γ ⊩s σ : Δ }} ->
+Lemma glu_rel_sub_wf_sub {P} (pred_P : PredicativeSig P) : forall {sts sts' Γ σ Δ},
+    glu_rel_sub pred_P Γ sts σ Δ sts' ->
+    (* {{ Γ ⊩s σ : Δ }} -> *)
     {{ Γ ⊢s σ : Δ }}.
 Proof.
   intros * [SbΓ [SbΔ]].
   destruct_conjs.
-  assert (exists env_relΓ, {{ EF Γ ≈ Γ ∈ per_ctx_env ↘ env_relΓ }}) as [env_relΓ] by mauto 3.
+  assert (exists env_relΓ, {{ EF Γ ≈ Γ ∈ per_ctx_env pred_P ↘ env_relΓ }}) as [env_relΓ] by mauto 3.
   assert (exists ρ ρ', initial_env Γ ρ /\ initial_env Γ ρ' /\ {{ Dom ρ ≈ ρ' ∈ env_relΓ }}) as [ρ] by mauto 3 using per_ctx_then_per_env_initial_env.
   destruct_conjs.
   functional_initial_env_rewrite_clear.
@@ -1444,8 +922,8 @@ Hint Resolve glu_rel_sub_wf_sub : mcpts.
 
 Ltac saturate_glu_typ_from_el1 :=
   match goal with
-  | H : glu_sort_elem _ _ ?El _, H1 : ?El _ _ _ _ |- _ =>
-      pose proof (glu_sort_elem_trm_typ _ _ _ _ H _ _ _ _ H1);
+  | H : glu_sort_elem _ _ _ ?exp_rel _, H1 : ?exp_rel _ _ _ _ |- _ =>
+      pose proof (glu_sort_elem_trm_typ _ _ _ _ _ H _ _ _ _ H1);
       fail_if_dup
   end.
 
@@ -1453,44 +931,51 @@ Ltac saturate_glu_typ_from_el :=
   fail_if_dup;
   repeat saturate_glu_typ_from_el1.
 
-Ltac unify_glu_sort_lvl1 i :=
-  match goal with
-  | H1 : glu_sort_elem _ _ ?El _, H2 : glu_sort_elem i ?P _ _, H3 : ?P _ _, H4 : ?El _ _ _ _
-    |- _ =>
-      pose proof (glu_sort_elem_exp_conv' H1 H2 H4 H3);
-      fail_if_dup
-  end.
 
-Ltac unify_glu_sort_lvl i :=
-  fail_if_dup;
-  repeat unify_glu_sort_lvl1 i.
+(* The proof `glu_univ_elem_exp_conv'` does not translate since it relies on cumulativity, but it would actually solve some problems if we could translate it somehow *)
 
-Ltac apply_glu_rel_judge :=
+
+
+(* Ltac unify_glu_univ_lvl1 i := *)
+(*   match goal with *)
+(*   | H1 : glu_univ_elem _ _ ?El _, H2 : glu_univ_elem i ?P _ _, H3 : ?P _ _, H4 : ?El _ _ _ _ *)
+(*     |- _ => *)
+(*       pose proof (glu_univ_elem_exp_conv' H1 H2 H4 H3); *)
+(*       fail_if_dup *)
+(*   end. *)
+
+(* Ltac unify_glu_univ_lvl i := *)
+(*   fail_if_dup; *)
+(*   repeat unify_glu_univ_lvl1 i. *)
+
+Ltac apply_glu_rel_judge P :=
   destruct_glu_rel_typ_with_sub;
   destruct_glu_rel_exp_with_sub;
   destruct_glu_rel_sub_with_sub;
   simplify_evals;
-  match_by_head glu_sort_elem ltac:(fun H => directed invert_glu_sort_elem H);
-  handle_functional_glu_sort_elem;
+  match_by_head (@glu_sort_elem P) ltac:(fun H => directed invert_glu_sort_elem H);
+  handle_functional_glu_sort_elem P;
   unfold sort_glu_exp_pred' in *;
   destruct_conjs;
   clear_dups.
 
 
-Lemma glu_rel_exp_preserves_lvl : forall Γ Sb M A i,
-    {{ EG Γ ∈ glu_ctx_env ↘ Sb }} ->
+Lemma glu_rel_exp_preserves_lvl {P} (pred_P : PredicativeSig P) : forall sts Γ Sb M A s,
+    {{ EG Γ ∈ glu_ctx_env pred_P sts ↘ Sb }} ->
     (forall Δ σ ρ,
         {{ Δ ⊢s σ ® ρ ∈ Sb }} ->
-        glu_rel_exp_with_sub i Δ M A σ ρ) ->
-    {{ Γ ⊢ A : Type@i }}.
+        glu_rel_exp_with_sub pred_P s Δ M A σ ρ) ->
+    {{ Γ ⊢ A : Sort@s }}.
 Proof.
   intros.
-  assert (exists env_relΓ, {{ EF Γ ≈ Γ ∈ per_ctx_env ↘ env_relΓ }}) as [env_relΓ] by mauto 3.
+  assert (exists env_relΓ, {{ EF Γ ≈ Γ ∈ per_ctx_env pred_P ↘ env_relΓ }}) as [env_relΓ] by mauto 3.
   assert (exists ρ ρ', initial_env Γ ρ /\ initial_env Γ ρ' /\ {{ Dom ρ ≈ ρ' ∈ env_relΓ }}) as [ρ] by mauto 3 using per_ctx_then_per_env_initial_env.
   destruct_conjs.
   functional_initial_env_rewrite_clear.
   assert {{ Γ ⊢s Id ® ρ ∈ Sb }} by (eapply initial_env_glu_rel_exp; mauto 3).
-  destruct_glu_rel_exp_with_sub.
+  assert (glu_rel_exp_with_sub pred_P s Γ M A {{{ Id }}} ρ) by mauto 2.
+  dependent destruction H4.
+  (* destruct_glu_rel_exp_with_sub. *)
   saturate_glu_typ_from_el.
   saturate_glu_info.
   mauto 3.
@@ -1503,9 +988,11 @@ Hint Resolve glu_rel_exp_preserves_lvl : mcpts.
 
 Ltac saturate_syn_judge1 :=
   match goal with
-  | H : {{ ^?Γ ⊩ ^?M : ^?A }} |- _ =>
+  | H : (glu_rel_exp ?pred_P ?Γ ?sts ?M ?A) |- _ =>
+      (* | H : {{ ⟪ ?pred_P ⟫ ^?Γ : ^?sts ⊩ ^?M : ^?A }} |- _ => *)
       assert {{ Γ ⊢ M : A }} by mauto; fail_if_dup
-  | H : {{ ^?Γ ⊩s ^?τ : ^?Γ' }} |- _ =>
+  | H : (glu_rel_sub ?pred_P ?Γ ?sts ?τ ?Γ' ?sts') |- _ =>
+    (* | H : {{ ⟪ ?pred_P ⟫ ^?Γ : ^?sts ⊩s ^?τ : ^?Γ' }} |- _ => *)
       assert {{ Γ ⊢s τ : Γ' }} by mauto; fail_if_dup
   end.
 
@@ -1515,9 +1002,11 @@ Ltac saturate_syn_judge1 :=
 
 Ltac invert_sem_judge1 :=
   match goal with
-  | H : {{ ^?Γ ⊩ ^?M : ^?A }} |- _ =>
+  | H : (glu_rel_exp ?pred_P ?Γ ?sts ?M ?A) |- _ =>
+  (* | H : {{ ^?Γ ⊩ ^?M : ^?A }} |- _ => *)
       invert_glu_rel_exp H
-  | H : {{ ^?Γ ⊩s ^?τ : ^?Γ' }} |- _ =>
+  | H : (glu_rel_sub ?pred_P ?Γ ?sts ?τ ?Γ' ?sts') |- _ =>                         
+  (* | H : {{ ^?Γ ⊩s ^?τ : ^?Γ' }} |- _ => *)
       invert_glu_rel_sub H
   end.
 
